Updated examples.

tests/AddDelay.bpl
@@ -37,13 +37,31 @@ procedure Delay#anon$2#2()
   var i: int;
   assume true;
 }
+procedure Net#init#3()
+  modifies C, R, M, St;
+{
+  var ActorParam#del#k: int;
+  assume C[Net#a] == 0;
+  assume R[Net#a] == 0;
+  assume C[Net#b] == 0;
+  assume R[Net#b] == 0;
+  assume C[Net#c] == 0;
+  assume R[Net#c] == 0;
+  assume C[Net#d] == 0;
+  assume R[Net#d] == 0;
+  assume ActorParam#del#k == 0;
+  M[Net#b][R[Net#b] + C[Net#b]] := ActorParam#del#k;
+  C[Net#b] := C[Net#b] + 1;
+  assert {:msg "  15.3: Network initialization might not establish the network invariant"} C[Net#b] == 1;
+  assert {:msg "  16.3: Network initialization might not establish the network invariant"} M[Net#b][R[Net#b]] == M[Net#c][R[Net#c] - 1];
+}
 const unique Net#add: Actor;
 const unique Net#del: Actor;
 const unique Net#a: Chan (int);
 const unique Net#b: Chan (int);
 const unique Net#c: Chan (int);
 const unique Net#d: Chan (int);
-procedure Net#anon$3#entry#3()
+procedure Net#anon$3#entry#4()
   modifies C, R, M, St;
 {
   assume C#init[Net#a] == 1;
@@ -56,39 +74,33 @@ procedure Net#anon$3#entry#3()
   assume C#init == C;
   assume C[Net#b] == 1;
   assume M[Net#b][R[Net#b]] == M[Net#c][R[Net#c] - 1];
-  assert {:msg "  Channel invariant might not hold on action entry (generated #0 )"} (forall idx$: int :: 
-    (0 <= idx$) && (idx$ < ((R[Net#b] + C[Net#b]) - 1)) ==> (M[Net#b][(idx$ + 1) - 0] == M[Net#d][idx$ - 0])
+  assert {:msg "  Channel invariant might not hold on action entry (generated #0)"} 0 <= R[Net#a];
+  assert {:msg "  Channel invariant might not hold on action entry (generated #1)"} 0 <= C[Net#a];
+  assert {:msg "  Channel invariant might not hold on action entry (generated #2)"} (R[Net#a] + C[Net#a]) == C#init[Net#a];
+  assert {:msg "  Channel invariant might not hold on action entry (generated #3)"} 0 <= R[Net#b];
+  assert {:msg "  Channel invariant might not hold on action entry (generated #4)"} 0 <= C[Net#b];
+  assert {:msg "  Channel invariant might not hold on action entry (generated #5)"} 0 <= R[Net#c];
+  assert {:msg "  Channel invariant might not hold on action entry (generated #6)"} 0 <= C[Net#c];
+  assert {:msg "  Channel invariant might not hold on action entry (generated #7)"} R[Net#c] == 0;
+  assert {:msg "  Channel invariant might not hold on action entry (generated #8)"} 0 <= R[Net#d];
+  assert {:msg "  Channel invariant might not hold on action entry (generated #9)"} 0 <= C[Net#d];
+  assert {:msg "  Channel invariant might not hold on action entry (generated #10)"} R[Net#a] == (R[Net#c] + C[Net#c]);
+  assert {:msg "  Channel invariant might not hold on action entry (generated #11)"} R[Net#b] == (R[Net#c] + C[Net#c]);
+  assert {:msg "  Channel invariant might not hold on action entry (generated #12)"} R[Net#a] == (R[Net#d] + C[Net#d]);
+  assert {:msg "  Channel invariant might not hold on action entry (generated #13)"} R[Net#b] == (R[Net#d] + C[Net#d]);
+  assert {:msg "  Channel invariant might not hold on action entry (generated #14)"} R[Net#d] == ((R[Net#b] + C[Net#b]) - 1);
+  assert {:msg "  Channel invariant might not hold on action entry (generated #15)"} (forall idx$: int :: 
+    (0 <= idx$) && (idx$ < (R[Net#c] + C[Net#c])) ==> (M[Net#c][idx$] == (M[Net#a][idx$] + M[Net#b][idx$]))
   );
-  assert {:msg "  Channel invariant might not hold on action entry (generated #1 )"} R[Net#d] == ((R[Net#b] + C[Net#b]) - 1);
-  assert {:msg "  Channel invariant might not hold on action entry (generated #2 )"} (forall idx$: int :: 
-    (0 <= idx$) && (idx$ < (R[Net#d] + C[Net#d])) ==> (M[Net#d][idx$ - 0] == (M[Net#a][idx$ - 0] + M[Net#b][idx$ - 0]))
+  assert {:msg "  Channel invariant might not hold on action entry (generated #16)"} (forall idx$: int :: 
+    (0 <= idx$) && (idx$ < (R[Net#d] + C[Net#d])) ==> (M[Net#d][idx$] == (M[Net#a][idx$] + M[Net#b][idx$]))
   );
-  assert {:msg "  Channel invariant might not hold on action entry (generated #3 )"} R[Net#b] == (R[Net#d] + C[Net#d]);
-  assert {:msg "  Channel invariant might not hold on action entry (generated #4 )"} (forall idx$: int :: 
-    (0 <= idx$) && (idx$ < (R[Net#c] + C[Net#c])) ==> (M[Net#c][idx$ - 0] == (M[Net#a][idx$ - 0] + M[Net#b][idx$ - 0]))
+  assert {:msg "  Channel invariant might not hold on action entry (generated #17)"} (forall idx$: int :: 
+    (1 <= idx$) && (idx$ < (R[Net#b] + C[Net#b])) ==> (M[Net#b][idx$] == M[Net#d][idx$ - 1])
   );
-  assert {:msg "  Channel invariant might not hold on action entry (generated #5 )"} R[Net#b] == (R[Net#c] + C[Net#c]);
-  assert {:msg "  Channel invariant might not hold on action entry (generated #6 )"} (forall idx$: int :: 
-    (0 <= idx$) && (idx$ < (R[Net#d] + C[Net#d])) ==> (M[Net#d][idx$ - 0] == (M[Net#a][idx$ - 0] + M[Net#b][idx$ - 0]))
-  );
-  assert {:msg "  Channel invariant might not hold on action entry (generated #7 )"} R[Net#a] == (R[Net#d] + C[Net#d]);
-  assert {:msg "  Channel invariant might not hold on action entry (generated #8 )"} (forall idx$: int :: 
-    (0 <= idx$) && (idx$ < (R[Net#c] + C[Net#c])) ==> (M[Net#c][idx$ - 0] == (M[Net#a][idx$ - 0] + M[Net#b][idx$ - 0]))
-  );
-  assert {:msg "  Channel invariant might not hold on action entry (generated #9 )"} R[Net#a] == (R[Net#c] + C[Net#c]);
-  assert {:msg "  Channel invariant might not hold on action entry (generated #10 )"} 0 <= C[Net#d];
-  assert {:msg "  Channel invariant might not hold on action entry (generated #11 )"} 0 <= R[Net#d];
-  assert {:msg "  Channel invariant might not hold on action entry (generated #12 )"} R[Net#c] == 0;
-  assert {:msg "  Channel invariant might not hold on action entry (generated #13 )"} 0 <= C[Net#c];
-  assert {:msg "  Channel invariant might not hold on action entry (generated #14 )"} 0 <= R[Net#c];
-  assert {:msg "  Channel invariant might not hold on action entry (generated #15 )"} 0 <= C[Net#b];
-  assert {:msg "  Channel invariant might not hold on action entry (generated #16 )"} 0 <= R[Net#b];
-  assert {:msg "  Channel invariant might not hold on action entry (generated #17 )"} (R[Net#a] + C[Net#a]) == C#init[Net#a];
-  assert {:msg "  Channel invariant might not hold on action entry (generated #18 )"} 0 <= C[Net#a];
-  assert {:msg "  Channel invariant might not hold on action entry (generated #19 )"} 0 <= R[Net#a];
   assert {:msg "  18.3: Channel invariant might not hold on action entry"} M[Net#b][0] == M[Net#c][-1];
 }
-procedure Net#anon$3#Add#anon$0#4()
+procedure Net#anon$3#Add#anon$0#5()
   modifies C, R, M, St;
 {
   var St#next: State;
@@ -97,36 +109,30 @@ procedure Net#anon$3#Add#anon$0#4()
   assume C#init[Net#a] == 1;
   assume C#init[Net#c] == 0;
   assume C#init[Net#d] == 0;
-  assume (forall idx$: int :: 
-    (0 <= idx$) && (idx$ < ((R[Net#b] + C[Net#b]) - 1)) ==> (M[Net#b][(idx$ + 1) - 0] == M[Net#d][idx$ - 0])
-  );
+  assume 0 <= R[Net#a];
+  assume 0 <= C[Net#a];
+  assume (R[Net#a] + C[Net#a]) == C#init[Net#a];
+  assume 0 <= R[Net#b];
+  assume 0 <= C[Net#b];
+  assume 0 <= R[Net#c];
+  assume 0 <= C[Net#c];
+  assume R[Net#c] == 0;
+  assume 0 <= R[Net#d];
+  assume 0 <= C[Net#d];
+  assume R[Net#a] == (R[Net#c] + C[Net#c]);
+  assume R[Net#b] == (R[Net#c] + C[Net#c]);
+  assume R[Net#a] == (R[Net#d] + C[Net#d]);
+  assume R[Net#b] == (R[Net#d] + C[Net#d]);
   assume R[Net#d] == ((R[Net#b] + C[Net#b]) - 1);
   assume (forall idx$: int :: 
-    (0 <= idx$) && (idx$ < (R[Net#d] + C[Net#d])) ==> (M[Net#d][idx$ - 0] == (M[Net#a][idx$ - 0] + M[Net#b][idx$ - 0]))
+    (0 <= idx$) && (idx$ < (R[Net#c] + C[Net#c])) ==> (M[Net#c][idx$] == (M[Net#a][idx$] + M[Net#b][idx$]))
   );
-  assume R[Net#b] == (R[Net#d] + C[Net#d]);
   assume (forall idx$: int :: 
-    (0 <= idx$) && (idx$ < (R[Net#c] + C[Net#c])) ==> (M[Net#c][idx$ - 0] == (M[Net#a][idx$ - 0] + M[Net#b][idx$ - 0]))
+    (0 <= idx$) && (idx$ < (R[Net#d] + C[Net#d])) ==> (M[Net#d][idx$] == (M[Net#a][idx$] + M[Net#b][idx$]))
   );
-  assume R[Net#b] == (R[Net#c] + C[Net#c]);
   assume (forall idx$: int :: 
-    (0 <= idx$) && (idx$ < (R[Net#d] + C[Net#d])) ==> (M[Net#d][idx$ - 0] == (M[Net#a][idx$ - 0] + M[Net#b][idx$ - 0]))
+    (1 <= idx$) && (idx$ < (R[Net#b] + C[Net#b])) ==> (M[Net#b][idx$] == M[Net#d][idx$ - 1])
   );
-  assume R[Net#a] == (R[Net#d] + C[Net#d]);
-  assume (forall idx$: int :: 
-    (0 <= idx$) && (idx$ < (R[Net#c] + C[Net#c])) ==> (M[Net#c][idx$ - 0] == (M[Net#a][idx$ - 0] + M[Net#b][idx$ - 0]))
-  );
-  assume R[Net#a] == (R[Net#c] + C[Net#c]);
-  assume 0 <= C[Net#d];
-  assume 0 <= R[Net#d];
-  assume R[Net#c] == 0;
-  assume 0 <= C[Net#c];
-  assume 0 <= R[Net#c];
-  assume 0 <= C[Net#b];
-  assume 0 <= R[Net#b];
-  assume (R[Net#a] + C[Net#a]) == C#init[Net#a];
-  assume 0 <= C[Net#a];
-  assume 0 <= R[Net#a];
   assume M[Net#b][0] == M[Net#c][-1];
   assume true;
   assume (1 <= C[Net#a]) && (1 <= C[Net#b]);
@@ -140,39 +146,33 @@ procedure Net#anon$3#Add#anon$0#4()
   C[Net#c] := C[Net#c] + 1;
   M[Net#d][R[Net#d] + C[Net#d]] := in1#i + in2#j;
   C[Net#d] := C[Net#d] + 1;
-  assert {:msg "  Sub-actor action at 3.3 might not preserve the channel invariant (generated #20)"} (forall idx$: int :: 
-    (0 <= idx$) && (idx$ < ((R[Net#b] + C[Net#b]) - 1)) ==> (M[Net#b][(idx$ + 1) - 0] == M[Net#d][idx$ - 0])
+  assert {:msg "  Sub-actor action at 3.3 might not preserve the channel invariant (generated #18)"} 0 <= R[Net#a];
+  assert {:msg "  Sub-actor action at 3.3 might not preserve the channel invariant (generated #19)"} 0 <= C[Net#a];
+  assert {:msg "  Sub-actor action at 3.3 might not preserve the channel invariant (generated #20)"} (R[Net#a] + C[Net#a]) == C#init[Net#a];
+  assert {:msg "  Sub-actor action at 3.3 might not preserve the channel invariant (generated #21)"} 0 <= R[Net#b];
+  assert {:msg "  Sub-actor action at 3.3 might not preserve the channel invariant (generated #22)"} 0 <= C[Net#b];
+  assert {:msg "  Sub-actor action at 3.3 might not preserve the channel invariant (generated #23)"} 0 <= R[Net#c];
+  assert {:msg "  Sub-actor action at 3.3 might not preserve the channel invariant (generated #24)"} 0 <= C[Net#c];
+  assert {:msg "  Sub-actor action at 3.3 might not preserve the channel invariant (generated #25)"} R[Net#c] == 0;
+  assert {:msg "  Sub-actor action at 3.3 might not preserve the channel invariant (generated #26)"} 0 <= R[Net#d];
+  assert {:msg "  Sub-actor action at 3.3 might not preserve the channel invariant (generated #27)"} 0 <= C[Net#d];
+  assert {:msg "  Sub-actor action at 3.3 might not preserve the channel invariant (generated #28)"} R[Net#a] == (R[Net#c] + C[Net#c]);
+  assert {:msg "  Sub-actor action at 3.3 might not preserve the channel invariant (generated #29)"} R[Net#b] == (R[Net#c] + C[Net#c]);
+  assert {:msg "  Sub-actor action at 3.3 might not preserve the channel invariant (generated #30)"} R[Net#a] == (R[Net#d] + C[Net#d]);
+  assert {:msg "  Sub-actor action at 3.3 might not preserve the channel invariant (generated #31)"} R[Net#b] == (R[Net#d] + C[Net#d]);
+  assert {:msg "  Sub-actor action at 3.3 might not preserve the channel invariant (generated #32)"} R[Net#d] == ((R[Net#b] + C[Net#b]) - 1);
+  assert {:msg "  Sub-actor action at 3.3 might not preserve the channel invariant (generated #33)"} (forall idx$: int :: 
+    (0 <= idx$) && (idx$ < (R[Net#c] + C[Net#c])) ==> (M[Net#c][idx$] == (M[Net#a][idx$] + M[Net#b][idx$]))
   );
-  assert {:msg "  Sub-actor action at 3.3 might not preserve the channel invariant (generated #21)"} R[Net#d] == ((R[Net#b] + C[Net#b]) - 1);
-  assert {:msg "  Sub-actor action at 3.3 might not preserve the channel invariant (generated #22)"} (forall idx$: int :: 
-    (0 <= idx$) && (idx$ < (R[Net#d] + C[Net#d])) ==> (M[Net#d][idx$ - 0] == (M[Net#a][idx$ - 0] + M[Net#b][idx$ - 0]))
+  assert {:msg "  Sub-actor action at 3.3 might not preserve the channel invariant (generated #34)"} (forall idx$: int :: 
+    (0 <= idx$) && (idx$ < (R[Net#d] + C[Net#d])) ==> (M[Net#d][idx$] == (M[Net#a][idx$] + M[Net#b][idx$]))
   );
-  assert {:msg "  Sub-actor action at 3.3 might not preserve the channel invariant (generated #23)"} R[Net#b] == (R[Net#d] + C[Net#d]);
-  assert {:msg "  Sub-actor action at 3.3 might not preserve the channel invariant (generated #24)"} (forall idx$: int :: 
-    (0 <= idx$) && (idx$ < (R[Net#c] + C[Net#c])) ==> (M[Net#c][idx$ - 0] == (M[Net#a][idx$ - 0] + M[Net#b][idx$ - 0]))
+  assert {:msg "  Sub-actor action at 3.3 might not preserve the channel invariant (generated #35)"} (forall idx$: int :: 
+    (1 <= idx$) && (idx$ < (R[Net#b] + C[Net#b])) ==> (M[Net#b][idx$] == M[Net#d][idx$ - 1])
   );
-  assert {:msg "  Sub-actor action at 3.3 might not preserve the channel invariant (generated #25)"} R[Net#b] == (R[Net#c] + C[Net#c]);
-  assert {:msg "  Sub-actor action at 3.3 might not preserve the channel invariant (generated #26)"} (forall idx$: int :: 
-    (0 <= idx$) && (idx$ < (R[Net#d] + C[Net#d])) ==> (M[Net#d][idx$ - 0] == (M[Net#a][idx$ - 0] + M[Net#b][idx$ - 0]))
-  );
-  assert {:msg "  Sub-actor action at 3.3 might not preserve the channel invariant (generated #27)"} R[Net#a] == (R[Net#d] + C[Net#d]);
-  assert {:msg "  Sub-actor action at 3.3 might not preserve the channel invariant (generated #28)"} (forall idx$: int :: 
-    (0 <= idx$) && (idx$ < (R[Net#c] + C[Net#c])) ==> (M[Net#c][idx$ - 0] == (M[Net#a][idx$ - 0] + M[Net#b][idx$ - 0]))
-  );
-  assert {:msg "  Sub-actor action at 3.3 might not preserve the channel invariant (generated #29)"} R[Net#a] == (R[Net#c] + C[Net#c]);
-  assert {:msg "  Sub-actor action at 3.3 might not preserve the channel invariant (generated #30)"} 0 <= C[Net#d];
-  assert {:msg "  Sub-actor action at 3.3 might not preserve the channel invariant (generated #31)"} 0 <= R[Net#d];
-  assert {:msg "  Sub-actor action at 3.3 might not preserve the channel invariant (generated #32)"} R[Net#c] == 0;
-  assert {:msg "  Sub-actor action at 3.3 might not preserve the channel invariant (generated #33)"} 0 <= C[Net#c];
-  assert {:msg "  Sub-actor action at 3.3 might not preserve the channel invariant (generated #34)"} 0 <= R[Net#c];
-  assert {:msg "  Sub-actor action at 3.3 might not preserve the channel invariant (generated #35)"} 0 <= C[Net#b];
-  assert {:msg "  Sub-actor action at 3.3 might not preserve the channel invariant (generated #36)"} 0 <= R[Net#b];
-  assert {:msg "  Sub-actor action at 3.3 might not preserve the channel invariant (generated #37)"} (R[Net#a] + C[Net#a]) == C#init[Net#a];
-  assert {:msg "  Sub-actor action at 3.3 might not preserve the channel invariant (generated #38)"} 0 <= C[Net#a];
-  assert {:msg "  Sub-actor action at 3.3 might not preserve the channel invariant (generated #39)"} 0 <= R[Net#a];
   assert {:msg "  18.3: Sub-actor action at 3.3 might not preserve the channel invariant"} M[Net#b][0] == M[Net#c][-1];
 }
-procedure Net#anon$3#Delay#anon$2#5()
+procedure Net#anon$3#Delay#anon$2#6()
   modifies C, R, M, St;
 {
   var ActorParam#k: int;
@@ -182,36 +182,30 @@ procedure Net#anon$3#Delay#anon$2#5()
   assume C#init[Net#a] == 1;
   assume C#init[Net#c] == 0;
   assume C#init[Net#d] == 0;
-  assume (forall idx$: int :: 
-    (0 <= idx$) && (idx$ < ((R[Net#b] + C[Net#b]) - 1)) ==> (M[Net#b][(idx$ + 1) - 0] == M[Net#d][idx$ - 0])
-  );
+  assume 0 <= R[Net#a];
+  assume 0 <= C[Net#a];
+  assume (R[Net#a] + C[Net#a]) == C#init[Net#a];
+  assume 0 <= R[Net#b];
+  assume 0 <= C[Net#b];
+  assume 0 <= R[Net#c];
+  assume 0 <= C[Net#c];
+  assume R[Net#c] == 0;
+  assume 0 <= R[Net#d];
+  assume 0 <= C[Net#d];
+  assume R[Net#a] == (R[Net#c] + C[Net#c]);
+  assume R[Net#b] == (R[Net#c] + C[Net#c]);
+  assume R[Net#a] == (R[Net#d] + C[Net#d]);
+  assume R[Net#b] == (R[Net#d] + C[Net#d]);
   assume R[Net#d] == ((R[Net#b] + C[Net#b]) - 1);
   assume (forall idx$: int :: 
-    (0 <= idx$) && (idx$ < (R[Net#d] + C[Net#d])) ==> (M[Net#d][idx$ - 0] == (M[Net#a][idx$ - 0] + M[Net#b][idx$ - 0]))
+    (0 <= idx$) && (idx$ < (R[Net#c] + C[Net#c])) ==> (M[Net#c][idx$] == (M[Net#a][idx$] + M[Net#b][idx$]))
   );
-  assume R[Net#b] == (R[Net#d] + C[Net#d]);
   assume (forall idx$: int :: 
-    (0 <= idx$) && (idx$ < (R[Net#c] + C[Net#c])) ==> (M[Net#c][idx$ - 0] == (M[Net#a][idx$ - 0] + M[Net#b][idx$ - 0]))
+    (0 <= idx$) && (idx$ < (R[Net#d] + C[Net#d])) ==> (M[Net#d][idx$] == (M[Net#a][idx$] + M[Net#b][idx$]))
   );
-  assume R[Net#b] == (R[Net#c] + C[Net#c]);
   assume (forall idx$: int :: 
-    (0 <= idx$) && (idx$ < (R[Net#d] + C[Net#d])) ==> (M[Net#d][idx$ - 0] == (M[Net#a][idx$ - 0] + M[Net#b][idx$ - 0]))
+    (1 <= idx$) && (idx$ < (R[Net#b] + C[Net#b])) ==> (M[Net#b][idx$] == M[Net#d][idx$ - 1])
   );
-  assume R[Net#a] == (R[Net#d] + C[Net#d]);
-  assume (forall idx$: int :: 
-    (0 <= idx$) && (idx$ < (R[Net#c] + C[Net#c])) ==> (M[Net#c][idx$ - 0] == (M[Net#a][idx$ - 0] + M[Net#b][idx$ - 0]))
-  );
-  assume R[Net#a] == (R[Net#c] + C[Net#c]);
-  assume 0 <= C[Net#d];
-  assume 0 <= R[Net#d];
-  assume R[Net#c] == 0;
-  assume 0 <= C[Net#c];
-  assume 0 <= R[Net#c];
-  assume 0 <= C[Net#b];
-  assume 0 <= R[Net#b];
-  assume (R[Net#a] + C[Net#a]) == C#init[Net#a];
-  assume 0 <= C[Net#a];
-  assume 0 <= R[Net#a];
   assume M[Net#b][0] == M[Net#c][-1];
   assume true;
   assume 1 <= C[Net#d];
@@ -220,74 +214,62 @@ procedure Net#anon$3#Delay#anon$2#5()
   C[Net#d] := C[Net#d] - 1;
   M[Net#b][R[Net#b] + C[Net#b]] := in#i;
   C[Net#b] := C[Net#b] + 1;
-  assert {:msg "  Sub-actor action at 9.3 might not preserve the channel invariant (generated #40)"} (forall idx$: int :: 
-    (0 <= idx$) && (idx$ < ((R[Net#b] + C[Net#b]) - 1)) ==> (M[Net#b][(idx$ + 1) - 0] == M[Net#d][idx$ - 0])
+  assert {:msg "  Sub-actor action at 9.3 might not preserve the channel invariant (generated #36)"} 0 <= R[Net#a];
+  assert {:msg "  Sub-actor action at 9.3 might not preserve the channel invariant (generated #37)"} 0 <= C[Net#a];
+  assert {:msg "  Sub-actor action at 9.3 might not preserve the channel invariant (generated #38)"} (R[Net#a] + C[Net#a]) == C#init[Net#a];
+  assert {:msg "  Sub-actor action at 9.3 might not preserve the channel invariant (generated #39)"} 0 <= R[Net#b];
+  assert {:msg "  Sub-actor action at 9.3 might not preserve the channel invariant (generated #40)"} 0 <= C[Net#b];
+  assert {:msg "  Sub-actor action at 9.3 might not preserve the channel invariant (generated #41)"} 0 <= R[Net#c];
+  assert {:msg "  Sub-actor action at 9.3 might not preserve the channel invariant (generated #42)"} 0 <= C[Net#c];
+  assert {:msg "  Sub-actor action at 9.3 might not preserve the channel invariant (generated #43)"} R[Net#c] == 0;
+  assert {:msg "  Sub-actor action at 9.3 might not preserve the channel invariant (generated #44)"} 0 <= R[Net#d];
+  assert {:msg "  Sub-actor action at 9.3 might not preserve the channel invariant (generated #45)"} 0 <= C[Net#d];
+  assert {:msg "  Sub-actor action at 9.3 might not preserve the channel invariant (generated #46)"} R[Net#a] == (R[Net#c] + C[Net#c]);
+  assert {:msg "  Sub-actor action at 9.3 might not preserve the channel invariant (generated #47)"} R[Net#b] == (R[Net#c] + C[Net#c]);
+  assert {:msg "  Sub-actor action at 9.3 might not preserve the channel invariant (generated #48)"} R[Net#a] == (R[Net#d] + C[Net#d]);
+  assert {:msg "  Sub-actor action at 9.3 might not preserve the channel invariant (generated #49)"} R[Net#b] == (R[Net#d] + C[Net#d]);
+  assert {:msg "  Sub-actor action at 9.3 might not preserve the channel invariant (generated #50)"} R[Net#d] == ((R[Net#b] + C[Net#b]) - 1);
+  assert {:msg "  Sub-actor action at 9.3 might not preserve the channel invariant (generated #51)"} (forall idx$: int :: 
+    (0 <= idx$) && (idx$ < (R[Net#c] + C[Net#c])) ==> (M[Net#c][idx$] == (M[Net#a][idx$] + M[Net#b][idx$]))
   );
-  assert {:msg "  Sub-actor action at 9.3 might not preserve the channel invariant (generated #41)"} R[Net#d] == ((R[Net#b] + C[Net#b]) - 1);
-  assert {:msg "  Sub-actor action at 9.3 might not preserve the channel invariant (generated #42)"} (forall idx$: int :: 
-    (0 <= idx$) && (idx$ < (R[Net#d] + C[Net#d])) ==> (M[Net#d][idx$ - 0] == (M[Net#a][idx$ - 0] + M[Net#b][idx$ - 0]))
+  assert {:msg "  Sub-actor action at 9.3 might not preserve the channel invariant (generated #52)"} (forall idx$: int :: 
+    (0 <= idx$) && (idx$ < (R[Net#d] + C[Net#d])) ==> (M[Net#d][idx$] == (M[Net#a][idx$] + M[Net#b][idx$]))
   );
-  assert {:msg "  Sub-actor action at 9.3 might not preserve the channel invariant (generated #43)"} R[Net#b] == (R[Net#d] + C[Net#d]);
-  assert {:msg "  Sub-actor action at 9.3 might not preserve the channel invariant (generated #44)"} (forall idx$: int :: 
-    (0 <= idx$) && (idx$ < (R[Net#c] + C[Net#c])) ==> (M[Net#c][idx$ - 0] == (M[Net#a][idx$ - 0] + M[Net#b][idx$ - 0]))
+  assert {:msg "  Sub-actor action at 9.3 might not preserve the channel invariant (generated #53)"} (forall idx$: int :: 
+    (1 <= idx$) && (idx$ < (R[Net#b] + C[Net#b])) ==> (M[Net#b][idx$] == M[Net#d][idx$ - 1])
   );
-  assert {:msg "  Sub-actor action at 9.3 might not preserve the channel invariant (generated #45)"} R[Net#b] == (R[Net#c] + C[Net#c]);
-  assert {:msg "  Sub-actor action at 9.3 might not preserve the channel invariant (generated #46)"} (forall idx$: int :: 
-    (0 <= idx$) && (idx$ < (R[Net#d] + C[Net#d])) ==> (M[Net#d][idx$ - 0] == (M[Net#a][idx$ - 0] + M[Net#b][idx$ - 0]))
-  );
-  assert {:msg "  Sub-actor action at 9.3 might not preserve the channel invariant (generated #47)"} R[Net#a] == (R[Net#d] + C[Net#d]);
-  assert {:msg "  Sub-actor action at 9.3 might not preserve the channel invariant (generated #48)"} (forall idx$: int :: 
-    (0 <= idx$) && (idx$ < (R[Net#c] + C[Net#c])) ==> (M[Net#c][idx$ - 0] == (M[Net#a][idx$ - 0] + M[Net#b][idx$ - 0]))
-  );
-  assert {:msg "  Sub-actor action at 9.3 might not preserve the channel invariant (generated #49)"} R[Net#a] == (R[Net#c] + C[Net#c]);
-  assert {:msg "  Sub-actor action at 9.3 might not preserve the channel invariant (generated #50)"} 0 <= C[Net#d];
-  assert {:msg "  Sub-actor action at 9.3 might not preserve the channel invariant (generated #51)"} 0 <= R[Net#d];
-  assert {:msg "  Sub-actor action at 9.3 might not preserve the channel invariant (generated #52)"} R[Net#c] == 0;
-  assert {:msg "  Sub-actor action at 9.3 might not preserve the channel invariant (generated #53)"} 0 <= C[Net#c];
-  assert {:msg "  Sub-actor action at 9.3 might not preserve the channel invariant (generated #54)"} 0 <= R[Net#c];
-  assert {:msg "  Sub-actor action at 9.3 might not preserve the channel invariant (generated #55)"} 0 <= C[Net#b];
-  assert {:msg "  Sub-actor action at 9.3 might not preserve the channel invariant (generated #56)"} 0 <= R[Net#b];
-  assert {:msg "  Sub-actor action at 9.3 might not preserve the channel invariant (generated #57)"} (R[Net#a] + C[Net#a]) == C#init[Net#a];
-  assert {:msg "  Sub-actor action at 9.3 might not preserve the channel invariant (generated #58)"} 0 <= C[Net#a];
-  assert {:msg "  Sub-actor action at 9.3 might not preserve the channel invariant (generated #59)"} 0 <= R[Net#a];
   assert {:msg "  18.3: Sub-actor action at 9.3 might not preserve the channel invariant"} M[Net#b][0] == M[Net#c][-1];
 }
-procedure Net#anon$3#exit#6()
+procedure Net#anon$3#exit#7()
   modifies C, R, M, St;
 {
   assume C#init[Net#a] == 1;
   assume C#init[Net#c] == 0;
   assume C#init[Net#d] == 0;
-  assume (forall idx$: int :: 
-    (0 <= idx$) && (idx$ < ((R[Net#b] + C[Net#b]) - 1)) ==> (M[Net#b][(idx$ + 1) - 0] == M[Net#d][idx$ - 0])
-  );
+  assume 0 <= R[Net#a];
+  assume 0 <= C[Net#a];
+  assume (R[Net#a] + C[Net#a]) == C#init[Net#a];
+  assume 0 <= R[Net#b];
+  assume 0 <= C[Net#b];
+  assume 0 <= R[Net#c];
+  assume 0 <= C[Net#c];
+  assume R[Net#c] == 0;
+  assume 0 <= R[Net#d];
+  assume 0 <= C[Net#d];
+  assume R[Net#a] == (R[Net#c] + C[Net#c]);
+  assume R[Net#b] == (R[Net#c] + C[Net#c]);
+  assume R[Net#a] == (R[Net#d] + C[Net#d]);
+  assume R[Net#b] == (R[Net#d] + C[Net#d]);
   assume R[Net#d] == ((R[Net#b] + C[Net#b]) - 1);
   assume (forall idx$: int :: 
-    (0 <= idx$) && (idx$ < (R[Net#d] + C[Net#d])) ==> (M[Net#d][idx$ - 0] == (M[Net#a][idx$ - 0] + M[Net#b][idx$ - 0]))
+    (0 <= idx$) && (idx$ < (R[Net#c] + C[Net#c])) ==> (M[Net#c][idx$] == (M[Net#a][idx$] + M[Net#b][idx$]))
   );
-  assume R[Net#b] == (R[Net#d] + C[Net#d]);
   assume (forall idx$: int :: 
-    (0 <= idx$) && (idx$ < (R[Net#c] + C[Net#c])) ==> (M[Net#c][idx$ - 0] == (M[Net#a][idx$ - 0] + M[Net#b][idx$ - 0]))
+    (0 <= idx$) && (idx$ < (R[Net#d] + C[Net#d])) ==> (M[Net#d][idx$] == (M[Net#a][idx$] + M[Net#b][idx$]))
   );
-  assume R[Net#b] == (R[Net#c] + C[Net#c]);
   assume (forall idx$: int :: 
-    (0 <= idx$) && (idx$ < (R[Net#d] + C[Net#d])) ==> (M[Net#d][idx$ - 0] == (M[Net#a][idx$ - 0] + M[Net#b][idx$ - 0]))
+    (1 <= idx$) && (idx$ < (R[Net#b] + C[Net#b])) ==> (M[Net#b][idx$] == M[Net#d][idx$ - 1])
   );
-  assume R[Net#a] == (R[Net#d] + C[Net#d]);
-  assume (forall idx$: int :: 
-    (0 <= idx$) && (idx$ < (R[Net#c] + C[Net#c])) ==> (M[Net#c][idx$ - 0] == (M[Net#a][idx$ - 0] + M[Net#b][idx$ - 0]))
-  );
-  assume R[Net#a] == (R[Net#c] + C[Net#c]);
-  assume 0 <= C[Net#d];
-  assume 0 <= R[Net#d];
-  assume R[Net#c] == 0;
-  assume 0 <= C[Net#c];
-  assume 0 <= R[Net#c];
-  assume 0 <= C[Net#b];
-  assume 0 <= R[Net#b];
-  assume (R[Net#a] + C[Net#a]) == C#init[Net#a];
-  assume 0 <= C[Net#a];
-  assume 0 <= R[Net#a];
   assume M[Net#b][0] == M[Net#c][-1];
   assume !(((1 <= C[Net#a]) && (1 <= C[Net#b])) || (1 <= C[Net#d]));
   assert {:msg "  13.3: The network might leave unread tokens on channel a"} C[Net#a] == 0;
