tests/IIR.bpl
@@ -68,6 +68,36 @@ procedure rshift#anon$4#4()
   var i: int;
   assume true;
 }
+procedure iir#init#5()
+  modifies C, R, M, St;
+{
+  var ActorParam#del1#k: int;
+  var ActorParam#mul1#c: int;
+  var ActorParam#mul2#c: int;
+  var ActorParam#rsh1#s: int;
+  assume C[iir#a] == 0;
+  assume R[iir#a] == 0;
+  assume C[iir#b] == 0;
+  assume R[iir#b] == 0;
+  assume C[iir#c] == 0;
+  assume R[iir#c] == 0;
+  assume C[iir#d] == 0;
+  assume R[iir#d] == 0;
+  assume C[iir#e] == 0;
+  assume R[iir#e] == 0;
+  assume C[iir#f] == 0;
+  assume R[iir#f] == 0;
+  assume C[iir#g] == 0;
+  assume R[iir#g] == 0;
+  assume ActorParam#del1#k == 0;
+  M[iir#f][R[iir#f] + C[iir#f]] := ActorParam#del1#k;
+  C[iir#f] := C[iir#f] + 1;
+  assume ActorParam#mul1#c == 85;
+  assume ActorParam#mul2#c == 171;
+  assume ActorParam#rsh1#s == 8;
+  assert {:msg "  25.3: Network initialization might not establish the network invariant"} C[iir#f] == 1;
+  assert {:msg "  26.3: Network initialization might not establish the network invariant"} M[iir#f][R[iir#f]] == (171 * M[iir#g][R[iir#g] - 1]);
+}
 const unique iir#del1: Actor;
 const unique iir#mul1: Actor;
 const unique iir#mul2: Actor;
@@ -80,7 +110,7 @@ const unique iir#d: Chan (int);
 const unique iir#e: Chan (int);
 const unique iir#f: Chan (int);
 const unique iir#g: Chan (int);
-procedure iir#anon$5#entry#5()
+procedure iir#anon$5#entry#6()
   modifies C, R, M, St;
 {
   assume C#init[iir#a] == 1;
@@ -99,53 +129,50 @@ procedure iir#anon$5#entry#5()
   assume C#init == C;
   assume C[iir#f] == 1;
   assume M[iir#f][R[iir#f]] == (171 * M[iir#g][R[iir#g] - 1]);
-  assert {:msg "  Channel invariant might not hold on action entry (generated #0 )"} (forall idx$: int :: 
-    (0 <= idx$) && (idx$ < (R[iir#c] + C[iir#c])) ==> (M[iir#c][idx$ - 0] == (M[iir#b][idx$ - 0] + M[iir#f][idx$ - 0]))
+  assert {:msg "  Channel invariant might not hold on action entry (generated #0)"} 0 <= R[iir#a];
+  assert {:msg "  Channel invariant might not hold on action entry (generated #1)"} 0 <= C[iir#a];
+  assert {:msg "  Channel invariant might not hold on action entry (generated #2)"} (R[iir#a] + C[iir#a]) == C#init[iir#a];
+  assert {:msg "  Channel invariant might not hold on action entry (generated #3)"} 0 <= R[iir#b];
+  assert {:msg "  Channel invariant might not hold on action entry (generated #4)"} 0 <= C[iir#b];
+  assert {:msg "  Channel invariant might not hold on action entry (generated #5)"} 0 <= R[iir#c];
+  assert {:msg "  Channel invariant might not hold on action entry (generated #6)"} 0 <= C[iir#c];
+  assert {:msg "  Channel invariant might not hold on action entry (generated #7)"} 0 <= R[iir#d];
+  assert {:msg "  Channel invariant might not hold on action entry (generated #8)"} 0 <= C[iir#d];
+  assert {:msg "  Channel invariant might not hold on action entry (generated #9)"} 0 <= R[iir#e];
+  assert {:msg "  Channel invariant might not hold on action entry (generated #10)"} 0 <= C[iir#e];
+  assert {:msg "  Channel invariant might not hold on action entry (generated #11)"} 0 <= R[iir#f];
+  assert {:msg "  Channel invariant might not hold on action entry (generated #12)"} 0 <= C[iir#f];
+  assert {:msg "  Channel invariant might not hold on action entry (generated #13)"} 0 <= R[iir#g];
+  assert {:msg "  Channel invariant might not hold on action entry (generated #14)"} 0 <= C[iir#g];
+  assert {:msg "  Channel invariant might not hold on action entry (generated #15)"} R[iir#g] == 0;
+  assert {:msg "  Channel invariant might not hold on action entry (generated #16)"} R[iir#e] == ((R[iir#f] + C[iir#f]) - 1);
+  assert {:msg "  Channel invariant might not hold on action entry (generated #17)"} R[iir#a] == (R[iir#b] + C[iir#b]);
+  assert {:msg "  Channel invariant might not hold on action entry (generated #18)"} R[iir#d] == (R[iir#e] + C[iir#e]);
+  assert {:msg "  Channel invariant might not hold on action entry (generated #19)"} R[iir#c] == (R[iir#d] + C[iir#d]);
+  assert {:msg "  Channel invariant might not hold on action entry (generated #20)"} R[iir#c] == (R[iir#g] + C[iir#g]);
+  assert {:msg "  Channel invariant might not hold on action entry (generated #21)"} R[iir#b] == (R[iir#c] + C[iir#c]);
+  assert {:msg "  Channel invariant might not hold on action entry (generated #22)"} R[iir#f] == (R[iir#c] + C[iir#c]);
+  assert {:msg "  Channel invariant might not hold on action entry (generated #23)"} (forall idx$: int :: 
+    (1 <= idx$) && (idx$ < (R[iir#f] + C[iir#f])) ==> (M[iir#f][idx$] == M[iir#e][idx$ - 1])
   );
-  assert {:msg "  Channel invariant might not hold on action entry (generated #1 )"} R[iir#f] == (R[iir#c] + C[iir#c]);
-  assert {:msg "  Channel invariant might not hold on action entry (generated #2 )"} (forall idx$: int :: 
-    (0 <= idx$) && (idx$ < (R[iir#c] + C[iir#c])) ==> (M[iir#c][idx$ - 0] == (M[iir#b][idx$ - 0] + M[iir#f][idx$ - 0]))
+  assert {:msg "  Channel invariant might not hold on action entry (generated #24)"} (forall idx$: int :: 
+    (0 <= idx$) && (idx$ < (R[iir#b] + C[iir#b])) ==> (M[iir#b][idx$] == (85 * M[iir#a][idx$]))
   );
-  assert {:msg "  Channel invariant might not hold on action entry (generated #3 )"} R[iir#b] == (R[iir#c] + C[iir#c]);
-  assert {:msg "  Channel invariant might not hold on action entry (generated #4 )"} (forall idx$: int :: 
-    (0 <= idx$) && (idx$ < (R[iir#g] + C[iir#g])) ==> (M[iir#g][idx$ - 0] == AT#RShift(M[iir#c][idx$ - 0], 8))
+  assert {:msg "  Channel invariant might not hold on action entry (generated #25)"} (forall idx$: int :: 
+    (0 <= idx$) && (idx$ < (R[iir#e] + C[iir#e])) ==> (M[iir#e][idx$] == (171 * M[iir#d][idx$]))
   );
-  assert {:msg "  Channel invariant might not hold on action entry (generated #5 )"} R[iir#c] == (R[iir#g] + C[iir#g]);
-  assert {:msg "  Channel invariant might not hold on action entry (generated #6 )"} (forall idx$: int :: 
-    (0 <= idx$) && (idx$ < (R[iir#d] + C[iir#d])) ==> (M[iir#d][idx$ - 0] == AT#RShift(M[iir#c][idx$ - 0], 8))
+  assert {:msg "  Channel invariant might not hold on action entry (generated #26)"} (forall idx$: int :: 
+    (0 <= idx$) && (idx$ < (R[iir#d] + C[iir#d])) ==> (M[iir#d][idx$] == AT#RShift(M[iir#c][idx$], 8))
   );
-  assert {:msg "  Channel invariant might not hold on action entry (generated #7 )"} R[iir#c] == (R[iir#d] + C[iir#d]);
-  assert {:msg "  Channel invariant might not hold on action entry (generated #8 )"} (forall idx$: int :: 
-    (0 <= idx$) && (idx$ < (R[iir#e] + C[iir#e])) ==> (M[iir#e][idx$ - 0] == (171 * M[iir#d][idx$ - 0]))
+  assert {:msg "  Channel invariant might not hold on action entry (generated #27)"} (forall idx$: int :: 
+    (0 <= idx$) && (idx$ < (R[iir#g] + C[iir#g])) ==> (M[iir#g][idx$] == AT#RShift(M[iir#c][idx$], 8))
   );
-  assert {:msg "  Channel invariant might not hold on action entry (generated #9 )"} R[iir#d] == (R[iir#e] + C[iir#e]);
-  assert {:msg "  Channel invariant might not hold on action entry (generated #10 )"} (forall idx$: int :: 
-    (0 <= idx$) && (idx$ < (R[iir#b] + C[iir#b])) ==> (M[iir#b][idx$ - 0] == (85 * M[iir#a][idx$ - 0]))
+  assert {:msg "  Channel invariant might not hold on action entry (generated #28)"} (forall idx$: int :: 
+    (0 <= idx$) && (idx$ < (R[iir#c] + C[iir#c])) ==> (M[iir#c][idx$] == (M[iir#b][idx$] + M[iir#f][idx$]))
   );
-  assert {:msg "  Channel invariant might not hold on action entry (generated #11 )"} R[iir#a] == (R[iir#b] + C[iir#b]);
-  assert {:msg "  Channel invariant might not hold on action entry (generated #12 )"} (forall idx$: int :: 
-    (0 <= idx$) && (idx$ < ((R[iir#f] + C[iir#f]) - 1)) ==> (M[iir#f][(idx$ + 1) - 0] == M[iir#e][idx$ - 0])
-  );
-  assert {:msg "  Channel invariant might not hold on action entry (generated #13 )"} R[iir#e] == ((R[iir#f] + C[iir#f]) - 1);
-  assert {:msg "  Channel invariant might not hold on action entry (generated #14 )"} R[iir#g] == 0;
-  assert {:msg "  Channel invariant might not hold on action entry (generated #15 )"} 0 <= C[iir#g];
-  assert {:msg "  Channel invariant might not hold on action entry (generated #16 )"} 0 <= R[iir#g];
-  assert {:msg "  Channel invariant might not hold on action entry (generated #17 )"} 0 <= C[iir#f];
-  assert {:msg "  Channel invariant might not hold on action entry (generated #18 )"} 0 <= R[iir#f];
-  assert {:msg "  Channel invariant might not hold on action entry (generated #19 )"} 0 <= C[iir#e];
-  assert {:msg "  Channel invariant might not hold on action entry (generated #20 )"} 0 <= R[iir#e];
-  assert {:msg "  Channel invariant might not hold on action entry (generated #21 )"} 0 <= C[iir#d];
-  assert {:msg "  Channel invariant might not hold on action entry (generated #22 )"} 0 <= R[iir#d];
-  assert {:msg "  Channel invariant might not hold on action entry (generated #23 )"} 0 <= C[iir#c];
-  assert {:msg "  Channel invariant might not hold on action entry (generated #24 )"} 0 <= R[iir#c];
-  assert {:msg "  Channel invariant might not hold on action entry (generated #25 )"} 0 <= C[iir#b];
-  assert {:msg "  Channel invariant might not hold on action entry (generated #26 )"} 0 <= R[iir#b];
-  assert {:msg "  Channel invariant might not hold on action entry (generated #27 )"} (R[iir#a] + C[iir#a]) == C#init[iir#a];
-  assert {:msg "  Channel invariant might not hold on action entry (generated #28 )"} 0 <= C[iir#a];
-  assert {:msg "  Channel invariant might not hold on action entry (generated #29 )"} 0 <= R[iir#a];
   assert {:msg "  28.3: Channel invariant might not hold on action entry"} (171 * M[iir#g][-1]) == M[iir#f][0];
 }
-procedure iir#anon$5#delay#anon$2#6()
+procedure iir#anon$5#delay#anon$2#7()
   modifies C, R, M, St;
 {
   var ActorParam#k: int;
@@ -158,50 +185,47 @@ procedure iir#anon$5#delay#anon$2#6()
   assume C#init[iir#d] == 0;
   assume C#init[iir#e] == 0;
   assume C#init[iir#g] == 0;
-  assume (forall idx$: int :: 
-    (0 <= idx$) && (idx$ < (R[iir#c] + C[iir#c])) ==> (M[iir#c][idx$ - 0] == (M[iir#b][idx$ - 0] + M[iir#f][idx$ - 0]))
-  );
+  assume 0 <= R[iir#a];
+  assume 0 <= C[iir#a];
+  assume (R[iir#a] + C[iir#a]) == C#init[iir#a];
+  assume 0 <= R[iir#b];
+  assume 0 <= C[iir#b];
+  assume 0 <= R[iir#c];
+  assume 0 <= C[iir#c];
+  assume 0 <= R[iir#d];
+  assume 0 <= C[iir#d];
+  assume 0 <= R[iir#e];
+  assume 0 <= C[iir#e];
+  assume 0 <= R[iir#f];
+  assume 0 <= C[iir#f];
+  assume 0 <= R[iir#g];
+  assume 0 <= C[iir#g];
+  assume R[iir#g] == 0;
+  assume R[iir#e] == ((R[iir#f] + C[iir#f]) - 1);
+  assume R[iir#a] == (R[iir#b] + C[iir#b]);
+  assume R[iir#d] == (R[iir#e] + C[iir#e]);
+  assume R[iir#c] == (R[iir#d] + C[iir#d]);
+  assume R[iir#c] == (R[iir#g] + C[iir#g]);
+  assume R[iir#b] == (R[iir#c] + C[iir#c]);
   assume R[iir#f] == (R[iir#c] + C[iir#c]);
   assume (forall idx$: int :: 
-    (0 <= idx$) && (idx$ < (R[iir#c] + C[iir#c])) ==> (M[iir#c][idx$ - 0] == (M[iir#b][idx$ - 0] + M[iir#f][idx$ - 0]))
+    (1 <= idx$) && (idx$ < (R[iir#f] + C[iir#f])) ==> (M[iir#f][idx$] == M[iir#e][idx$ - 1])
   );
-  assume R[iir#b] == (R[iir#c] + C[iir#c]);
   assume (forall idx$: int :: 
-    (0 <= idx$) && (idx$ < (R[iir#g] + C[iir#g])) ==> (M[iir#g][idx$ - 0] == AT#RShift(M[iir#c][idx$ - 0], 8))
+    (0 <= idx$) && (idx$ < (R[iir#b] + C[iir#b])) ==> (M[iir#b][idx$] == (85 * M[iir#a][idx$]))
   );
-  assume R[iir#c] == (R[iir#g] + C[iir#g]);
   assume (forall idx$: int :: 
-    (0 <= idx$) && (idx$ < (R[iir#d] + C[iir#d])) ==> (M[iir#d][idx$ - 0] == AT#RShift(M[iir#c][idx$ - 0], 8))
+    (0 <= idx$) && (idx$ < (R[iir#e] + C[iir#e])) ==> (M[iir#e][idx$] == (171 * M[iir#d][idx$]))
   );
-  assume R[iir#c] == (R[iir#d] + C[iir#d]);
   assume (forall idx$: int :: 
-    (0 <= idx$) && (idx$ < (R[iir#e] + C[iir#e])) ==> (M[iir#e][idx$ - 0] == (171 * M[iir#d][idx$ - 0]))
+    (0 <= idx$) && (idx$ < (R[iir#d] + C[iir#d])) ==> (M[iir#d][idx$] == AT#RShift(M[iir#c][idx$], 8))
   );
-  assume R[iir#d] == (R[iir#e] + C[iir#e]);
   assume (forall idx$: int :: 
-    (0 <= idx$) && (idx$ < (R[iir#b] + C[iir#b])) ==> (M[iir#b][idx$ - 0] == (85 * M[iir#a][idx$ - 0]))
+    (0 <= idx$) && (idx$ < (R[iir#g] + C[iir#g])) ==> (M[iir#g][idx$] == AT#RShift(M[iir#c][idx$], 8))
   );
-  assume R[iir#a] == (R[iir#b] + C[iir#b]);
   assume (forall idx$: int :: 
-    (0 <= idx$) && (idx$ < ((R[iir#f] + C[iir#f]) - 1)) ==> (M[iir#f][(idx$ + 1) - 0] == M[iir#e][idx$ - 0])
+    (0 <= idx$) && (idx$ < (R[iir#c] + C[iir#c])) ==> (M[iir#c][idx$] == (M[iir#b][idx$] + M[iir#f][idx$]))
   );
-  assume R[iir#e] == ((R[iir#f] + C[iir#f]) - 1);
-  assume R[iir#g] == 0;
-  assume 0 <= C[iir#g];
-  assume 0 <= R[iir#g];
-  assume 0 <= C[iir#f];
-  assume 0 <= R[iir#f];
-  assume 0 <= C[iir#e];
-  assume 0 <= R[iir#e];
-  assume 0 <= C[iir#d];
-  assume 0 <= R[iir#d];
-  assume 0 <= C[iir#c];
-  assume 0 <= R[iir#c];
-  assume 0 <= C[iir#b];
-  assume 0 <= R[iir#b];
-  assume (R[iir#a] + C[iir#a]) == C#init[iir#a];
-  assume 0 <= C[iir#a];
-  assume 0 <= R[iir#a];
   assume (171 * M[iir#g][-1]) == M[iir#f][0];
   assume true;
   assume 1 <= C[iir#e];
@@ -210,53 +234,50 @@ procedure iir#anon$5#delay#anon$2#6()
   C[iir#e] := C[iir#e] - 1;
   M[iir#f][R[iir#f] + C[iir#f]] := in#i;
   C[iir#f] := C[iir#f] + 1;
-  assert {:msg "  Sub-actor action at 9.3 might not preserve the channel invariant (generated #30)"} (forall idx$: int :: 
-    (0 <= idx$) && (idx$ < (R[iir#c] + C[iir#c])) ==> (M[iir#c][idx$ - 0] == (M[iir#b][idx$ - 0] + M[iir#f][idx$ - 0]))
-  );
-  assert {:msg "  Sub-actor action at 9.3 might not preserve the channel invariant (generated #31)"} R[iir#f] == (R[iir#c] + C[iir#c]);
-  assert {:msg "  Sub-actor action at 9.3 might not preserve the channel invariant (generated #32)"} (forall idx$: int :: 
-    (0 <= idx$) && (idx$ < (R[iir#c] + C[iir#c])) ==> (M[iir#c][idx$ - 0] == (M[iir#b][idx$ - 0] + M[iir#f][idx$ - 0]))
-  );
-  assert {:msg "  Sub-actor action at 9.3 might not preserve the channel invariant (generated #33)"} R[iir#b] == (R[iir#c] + C[iir#c]);
-  assert {:msg "  Sub-actor action at 9.3 might not preserve the channel invariant (generated #34)"} (forall idx$: int :: 
-    (0 <= idx$) && (idx$ < (R[iir#g] + C[iir#g])) ==> (M[iir#g][idx$ - 0] == AT#RShift(M[iir#c][idx$ - 0], 8))
-  );
-  assert {:msg "  Sub-actor action at 9.3 might not preserve the channel invariant (generated #35)"} R[iir#c] == (R[iir#g] + C[iir#g]);
-  assert {:msg "  Sub-actor action at 9.3 might not preserve the channel invariant (generated #36)"} (forall idx$: int :: 
-    (0 <= idx$) && (idx$ < (R[iir#d] + C[iir#d])) ==> (M[iir#d][idx$ - 0] == AT#RShift(M[iir#c][idx$ - 0], 8))
-  );
-  assert {:msg "  Sub-actor action at 9.3 might not preserve the channel invariant (generated #37)"} R[iir#c] == (R[iir#d] + C[iir#d]);
-  assert {:msg "  Sub-actor action at 9.3 might not preserve the channel invariant (generated #38)"} (forall idx$: int :: 
-    (0 <= idx$) && (idx$ < (R[iir#e] + C[iir#e])) ==> (M[iir#e][idx$ - 0] == (171 * M[iir#d][idx$ - 0]))
-  );
-  assert {:msg "  Sub-actor action at 9.3 might not preserve the channel invariant (generated #39)"} R[iir#d] == (R[iir#e] + C[iir#e]);
-  assert {:msg "  Sub-actor action at 9.3 might not preserve the channel invariant (generated #40)"} (forall idx$: int :: 
-    (0 <= idx$) && (idx$ < (R[iir#b] + C[iir#b])) ==> (M[iir#b][idx$ - 0] == (85 * M[iir#a][idx$ - 0]))
-  );
-  assert {:msg "  Sub-actor action at 9.3 might not preserve the channel invariant (generated #41)"} R[iir#a] == (R[iir#b] + C[iir#b]);
-  assert {:msg "  Sub-actor action at 9.3 might not preserve the channel invariant (generated #42)"} (forall idx$: int :: 
-    (0 <= idx$) && (idx$ < ((R[iir#f] + C[iir#f]) - 1)) ==> (M[iir#f][(idx$ + 1) - 0] == M[iir#e][idx$ - 0])
-  );
-  assert {:msg "  Sub-actor action at 9.3 might not preserve the channel invariant (generated #43)"} R[iir#e] == ((R[iir#f] + C[iir#f]) - 1);
+  assert {:msg "  Sub-actor action at 9.3 might not preserve the channel invariant (generated #29)"} 0 <= R[iir#a];
+  assert {:msg "  Sub-actor action at 9.3 might not preserve the channel invariant (generated #30)"} 0 <= C[iir#a];
+  assert {:msg "  Sub-actor action at 9.3 might not preserve the channel invariant (generated #31)"} (R[iir#a] + C[iir#a]) == C#init[iir#a];
+  assert {:msg "  Sub-actor action at 9.3 might not preserve the channel invariant (generated #32)"} 0 <= R[iir#b];
+  assert {:msg "  Sub-actor action at 9.3 might not preserve the channel invariant (generated #33)"} 0 <= C[iir#b];
+  assert {:msg "  Sub-actor action at 9.3 might not preserve the channel invariant (generated #34)"} 0 <= R[iir#c];
+  assert {:msg "  Sub-actor action at 9.3 might not preserve the channel invariant (generated #35)"} 0 <= C[iir#c];
+  assert {:msg "  Sub-actor action at 9.3 might not preserve the channel invariant (generated #36)"} 0 <= R[iir#d];
+  assert {:msg "  Sub-actor action at 9.3 might not preserve the channel invariant (generated #37)"} 0 <= C[iir#d];
+  assert {:msg "  Sub-actor action at 9.3 might not preserve the channel invariant (generated #38)"} 0 <= R[iir#e];
+  assert {:msg "  Sub-actor action at 9.3 might not preserve the channel invariant (generated #39)"} 0 <= C[iir#e];
+  assert {:msg "  Sub-actor action at 9.3 might not preserve the channel invariant (generated #40)"} 0 <= R[iir#f];
+  assert {:msg "  Sub-actor action at 9.3 might not preserve the channel invariant (generated #41)"} 0 <= C[iir#f];
+  assert {:msg "  Sub-actor action at 9.3 might not preserve the channel invariant (generated #42)"} 0 <= R[iir#g];
+  assert {:msg "  Sub-actor action at 9.3 might not preserve the channel invariant (generated #43)"} 0 <= C[iir#g];
   assert {:msg "  Sub-actor action at 9.3 might not preserve the channel invariant (generated #44)"} R[iir#g] == 0;
-  assert {:msg "  Sub-actor action at 9.3 might not preserve the channel invariant (generated #45)"} 0 <= C[iir#g];
-  assert {:msg "  Sub-actor action at 9.3 might not preserve the channel invariant (generated #46)"} 0 <= R[iir#g];
-  assert {:msg "  Sub-actor action at 9.3 might not preserve the channel invariant (generated #47)"} 0 <= C[iir#f];
-  assert {:msg "  Sub-actor action at 9.3 might not preserve the channel invariant (generated #48)"} 0 <= R[iir#f];
-  assert {:msg "  Sub-actor action at 9.3 might not preserve the channel invariant (generated #49)"} 0 <= C[iir#e];
-  assert {:msg "  Sub-actor action at 9.3 might not preserve the channel invariant (generated #50)"} 0 <= R[iir#e];
-  assert {:msg "  Sub-actor action at 9.3 might not preserve the channel invariant (generated #51)"} 0 <= C[iir#d];
-  assert {:msg "  Sub-actor action at 9.3 might not preserve the channel invariant (generated #52)"} 0 <= R[iir#d];
-  assert {:msg "  Sub-actor action at 9.3 might not preserve the channel invariant (generated #53)"} 0 <= C[iir#c];
-  assert {:msg "  Sub-actor action at 9.3 might not preserve the channel invariant (generated #54)"} 0 <= R[iir#c];
-  assert {:msg "  Sub-actor action at 9.3 might not preserve the channel invariant (generated #55)"} 0 <= C[iir#b];
-  assert {:msg "  Sub-actor action at 9.3 might not preserve the channel invariant (generated #56)"} 0 <= R[iir#b];
-  assert {:msg "  Sub-actor action at 9.3 might not preserve the channel invariant (generated #57)"} (R[iir#a] + C[iir#a]) == C#init[iir#a];
-  assert {:msg "  Sub-actor action at 9.3 might not preserve the channel invariant (generated #58)"} 0 <= C[iir#a];
-  assert {:msg "  Sub-actor action at 9.3 might not preserve the channel invariant (generated #59)"} 0 <= R[iir#a];
+  assert {:msg "  Sub-actor action at 9.3 might not preserve the channel invariant (generated #45)"} R[iir#e] == ((R[iir#f] + C[iir#f]) - 1);
+  assert {:msg "  Sub-actor action at 9.3 might not preserve the channel invariant (generated #46)"} R[iir#a] == (R[iir#b] + C[iir#b]);
+  assert {:msg "  Sub-actor action at 9.3 might not preserve the channel invariant (generated #47)"} R[iir#d] == (R[iir#e] + C[iir#e]);
+  assert {:msg "  Sub-actor action at 9.3 might not preserve the channel invariant (generated #48)"} R[iir#c] == (R[iir#d] + C[iir#d]);
+  assert {:msg "  Sub-actor action at 9.3 might not preserve the channel invariant (generated #49)"} R[iir#c] == (R[iir#g] + C[iir#g]);
+  assert {:msg "  Sub-actor action at 9.3 might not preserve the channel invariant (generated #50)"} R[iir#b] == (R[iir#c] + C[iir#c]);
+  assert {:msg "  Sub-actor action at 9.3 might not preserve the channel invariant (generated #51)"} R[iir#f] == (R[iir#c] + C[iir#c]);
+  assert {:msg "  Sub-actor action at 9.3 might not preserve the channel invariant (generated #52)"} (forall idx$: int :: 
+    (1 <= idx$) && (idx$ < (R[iir#f] + C[iir#f])) ==> (M[iir#f][idx$] == M[iir#e][idx$ - 1])
+  );
+  assert {:msg "  Sub-actor action at 9.3 might not preserve the channel invariant (generated #53)"} (forall idx$: int :: 
+    (0 <= idx$) && (idx$ < (R[iir#b] + C[iir#b])) ==> (M[iir#b][idx$] == (85 * M[iir#a][idx$]))
+  );
+  assert {:msg "  Sub-actor action at 9.3 might not preserve the channel invariant (generated #54)"} (forall idx$: int :: 
+    (0 <= idx$) && (idx$ < (R[iir#e] + C[iir#e])) ==> (M[iir#e][idx$] == (171 * M[iir#d][idx$]))
+  );
+  assert {:msg "  Sub-actor action at 9.3 might not preserve the channel invariant (generated #55)"} (forall idx$: int :: 
+    (0 <= idx$) && (idx$ < (R[iir#d] + C[iir#d])) ==> (M[iir#d][idx$] == AT#RShift(M[iir#c][idx$], 8))
+  );
+  assert {:msg "  Sub-actor action at 9.3 might not preserve the channel invariant (generated #56)"} (forall idx$: int :: 
+    (0 <= idx$) && (idx$ < (R[iir#g] + C[iir#g])) ==> (M[iir#g][idx$] == AT#RShift(M[iir#c][idx$], 8))
+  );
+  assert {:msg "  Sub-actor action at 9.3 might not preserve the channel invariant (generated #57)"} (forall idx$: int :: 
+    (0 <= idx$) && (idx$ < (R[iir#c] + C[iir#c])) ==> (M[iir#c][idx$] == (M[iir#b][idx$] + M[iir#f][idx$]))
+  );
   assert {:msg "  28.3: Sub-actor action at 9.3 might not preserve the channel invariant"} (171 * M[iir#g][-1]) == M[iir#f][0];
 }
-procedure iir#anon$5#mulc#anon$3#7()
+procedure iir#anon$5#mulc#anon$3#8()
   modifies C, R, M, St;
 {
   var ActorParam#c: int;
@@ -269,50 +290,47 @@ procedure iir#anon$5#mulc#anon$3#7()
   assume C#init[iir#d] == 0;
   assume C#init[iir#e] == 0;
   assume C#init[iir#g] == 0;
-  assume (forall idx$: int :: 
-    (0 <= idx$) && (idx$ < (R[iir#c] + C[iir#c])) ==> (M[iir#c][idx$ - 0] == (M[iir#b][idx$ - 0] + M[iir#f][idx$ - 0]))
-  );
+  assume 0 <= R[iir#a];
+  assume 0 <= C[iir#a];
+  assume (R[iir#a] + C[iir#a]) == C#init[iir#a];
+  assume 0 <= R[iir#b];
+  assume 0 <= C[iir#b];
+  assume 0 <= R[iir#c];
+  assume 0 <= C[iir#c];
+  assume 0 <= R[iir#d];
+  assume 0 <= C[iir#d];
+  assume 0 <= R[iir#e];
+  assume 0 <= C[iir#e];
+  assume 0 <= R[iir#f];
+  assume 0 <= C[iir#f];
+  assume 0 <= R[iir#g];
+  assume 0 <= C[iir#g];
+  assume R[iir#g] == 0;
+  assume R[iir#e] == ((R[iir#f] + C[iir#f]) - 1);
+  assume R[iir#a] == (R[iir#b] + C[iir#b]);
+  assume R[iir#d] == (R[iir#e] + C[iir#e]);
+  assume R[iir#c] == (R[iir#d] + C[iir#d]);
+  assume R[iir#c] == (R[iir#g] + C[iir#g]);
+  assume R[iir#b] == (R[iir#c] + C[iir#c]);
   assume R[iir#f] == (R[iir#c] + C[iir#c]);
   assume (forall idx$: int :: 
-    (0 <= idx$) && (idx$ < (R[iir#c] + C[iir#c])) ==> (M[iir#c][idx$ - 0] == (M[iir#b][idx$ - 0] + M[iir#f][idx$ - 0]))
+    (1 <= idx$) && (idx$ < (R[iir#f] + C[iir#f])) ==> (M[iir#f][idx$] == M[iir#e][idx$ - 1])
   );
-  assume R[iir#b] == (R[iir#c] + C[iir#c]);
   assume (forall idx$: int :: 
-    (0 <= idx$) && (idx$ < (R[iir#g] + C[iir#g])) ==> (M[iir#g][idx$ - 0] == AT#RShift(M[iir#c][idx$ - 0], 8))
+    (0 <= idx$) && (idx$ < (R[iir#b] + C[iir#b])) ==> (M[iir#b][idx$] == (85 * M[iir#a][idx$]))
   );
-  assume R[iir#c] == (R[iir#g] + C[iir#g]);
   assume (forall idx$: int :: 
-    (0 <= idx$) && (idx$ < (R[iir#d] + C[iir#d])) ==> (M[iir#d][idx$ - 0] == AT#RShift(M[iir#c][idx$ - 0], 8))
+    (0 <= idx$) && (idx$ < (R[iir#e] + C[iir#e])) ==> (M[iir#e][idx$] == (171 * M[iir#d][idx$]))
   );
-  assume R[iir#c] == (R[iir#d] + C[iir#d]);
   assume (forall idx$: int :: 
-    (0 <= idx$) && (idx$ < (R[iir#e] + C[iir#e])) ==> (M[iir#e][idx$ - 0] == (171 * M[iir#d][idx$ - 0]))
+    (0 <= idx$) && (idx$ < (R[iir#d] + C[iir#d])) ==> (M[iir#d][idx$] == AT#RShift(M[iir#c][idx$], 8))
   );
-  assume R[iir#d] == (R[iir#e] + C[iir#e]);
   assume (forall idx$: int :: 
-    (0 <= idx$) && (idx$ < (R[iir#b] + C[iir#b])) ==> (M[iir#b][idx$ - 0] == (85 * M[iir#a][idx$ - 0]))
+    (0 <= idx$) && (idx$ < (R[iir#g] + C[iir#g])) ==> (M[iir#g][idx$] == AT#RShift(M[iir#c][idx$], 8))
   );
-  assume R[iir#a] == (R[iir#b] + C[iir#b]);
   assume (forall idx$: int :: 
-    (0 <= idx$) && (idx$ < ((R[iir#f] + C[iir#f]) - 1)) ==> (M[iir#f][(idx$ + 1) - 0] == M[iir#e][idx$ - 0])
+    (0 <= idx$) && (idx$ < (R[iir#c] + C[iir#c])) ==> (M[iir#c][idx$] == (M[iir#b][idx$] + M[iir#f][idx$]))
   );
-  assume R[iir#e] == ((R[iir#f] + C[iir#f]) - 1);
-  assume R[iir#g] == 0;
-  assume 0 <= C[iir#g];
-  assume 0 <= R[iir#g];
-  assume 0 <= C[iir#f];
-  assume 0 <= R[iir#f];
-  assume 0 <= C[iir#e];
-  assume 0 <= R[iir#e];
-  assume 0 <= C[iir#d];
-  assume 0 <= R[iir#d];
-  assume 0 <= C[iir#c];
-  assume 0 <= R[iir#c];
-  assume 0 <= C[iir#b];
-  assume 0 <= R[iir#b];
-  assume (R[iir#a] + C[iir#a]) == C#init[iir#a];
-  assume 0 <= C[iir#a];
-  assume 0 <= R[iir#a];
   assume (171 * M[iir#g][-1]) == M[iir#f][0];
   assume true;
   assume 1 <= C[iir#a];
@@ -321,53 +339,50 @@ procedure iir#anon$5#mulc#anon$3#7()
   C[iir#a] := C[iir#a] - 1;
   M[iir#b][R[iir#b] + C[iir#b]] := ActorParam#c * in#i;
   C[iir#b] := C[iir#b] + 1;
-  assert {:msg "  Sub-actor action at 14.3 might not preserve the channel invariant (generated #60)"} (forall idx$: int :: 
-    (0 <= idx$) && (idx$ < (R[iir#c] + C[iir#c])) ==> (M[iir#c][idx$ - 0] == (M[iir#b][idx$ - 0] + M[iir#f][idx$ - 0]))
+  assert {:msg "  Sub-actor action at 14.3 might not preserve the channel invariant (generated #58)"} 0 <= R[iir#a];
+  assert {:msg "  Sub-actor action at 14.3 might not preserve the channel invariant (generated #59)"} 0 <= C[iir#a];
+  assert {:msg "  Sub-actor action at 14.3 might not preserve the channel invariant (generated #60)"} (R[iir#a] + C[iir#a]) == C#init[iir#a];
+  assert {:msg "  Sub-actor action at 14.3 might not preserve the channel invariant (generated #61)"} 0 <= R[iir#b];
+  assert {:msg "  Sub-actor action at 14.3 might not preserve the channel invariant (generated #62)"} 0 <= C[iir#b];
+  assert {:msg "  Sub-actor action at 14.3 might not preserve the channel invariant (generated #63)"} 0 <= R[iir#c];
+  assert {:msg "  Sub-actor action at 14.3 might not preserve the channel invariant (generated #64)"} 0 <= C[iir#c];
+  assert {:msg "  Sub-actor action at 14.3 might not preserve the channel invariant (generated #65)"} 0 <= R[iir#d];
+  assert {:msg "  Sub-actor action at 14.3 might not preserve the channel invariant (generated #66)"} 0 <= C[iir#d];
+  assert {:msg "  Sub-actor action at 14.3 might not preserve the channel invariant (generated #67)"} 0 <= R[iir#e];
+  assert {:msg "  Sub-actor action at 14.3 might not preserve the channel invariant (generated #68)"} 0 <= C[iir#e];
+  assert {:msg "  Sub-actor action at 14.3 might not preserve the channel invariant (generated #69)"} 0 <= R[iir#f];
+  assert {:msg "  Sub-actor action at 14.3 might not preserve the channel invariant (generated #70)"} 0 <= C[iir#f];
+  assert {:msg "  Sub-actor action at 14.3 might not preserve the channel invariant (generated #71)"} 0 <= R[iir#g];
+  assert {:msg "  Sub-actor action at 14.3 might not preserve the channel invariant (generated #72)"} 0 <= C[iir#g];
+  assert {:msg "  Sub-actor action at 14.3 might not preserve the channel invariant (generated #73)"} R[iir#g] == 0;
+  assert {:msg "  Sub-actor action at 14.3 might not preserve the channel invariant (generated #74)"} R[iir#e] == ((R[iir#f] + C[iir#f]) - 1);
+  assert {:msg "  Sub-actor action at 14.3 might not preserve the channel invariant (generated #75)"} R[iir#a] == (R[iir#b] + C[iir#b]);
+  assert {:msg "  Sub-actor action at 14.3 might not preserve the channel invariant (generated #76)"} R[iir#d] == (R[iir#e] + C[iir#e]);
+  assert {:msg "  Sub-actor action at 14.3 might not preserve the channel invariant (generated #77)"} R[iir#c] == (R[iir#d] + C[iir#d]);
+  assert {:msg "  Sub-actor action at 14.3 might not preserve the channel invariant (generated #78)"} R[iir#c] == (R[iir#g] + C[iir#g]);
+  assert {:msg "  Sub-actor action at 14.3 might not preserve the channel invariant (generated #79)"} R[iir#b] == (R[iir#c] + C[iir#c]);
+  assert {:msg "  Sub-actor action at 14.3 might not preserve the channel invariant (generated #80)"} R[iir#f] == (R[iir#c] + C[iir#c]);
+  assert {:msg "  Sub-actor action at 14.3 might not preserve the channel invariant (generated #81)"} (forall idx$: int :: 
+    (1 <= idx$) && (idx$ < (R[iir#f] + C[iir#f])) ==> (M[iir#f][idx$] == M[iir#e][idx$ - 1])
   );
-  assert {:msg "  Sub-actor action at 14.3 might not preserve the channel invariant (generated #61)"} R[iir#f] == (R[iir#c] + C[iir#c]);
-  assert {:msg "  Sub-actor action at 14.3 might not preserve the channel invariant (generated #62)"} (forall idx$: int :: 
-    (0 <= idx$) && (idx$ < (R[iir#c] + C[iir#c])) ==> (M[iir#c][idx$ - 0] == (M[iir#b][idx$ - 0] + M[iir#f][idx$ - 0]))
+  assert {:msg "  Sub-actor action at 14.3 might not preserve the channel invariant (generated #82)"} (forall idx$: int :: 
+    (0 <= idx$) && (idx$ < (R[iir#b] + C[iir#b])) ==> (M[iir#b][idx$] == (85 * M[iir#a][idx$]))
   );
-  assert {:msg "  Sub-actor action at 14.3 might not preserve the channel invariant (generated #63)"} R[iir#b] == (R[iir#c] + C[iir#c]);
-  assert {:msg "  Sub-actor action at 14.3 might not preserve the channel invariant (generated #64)"} (forall idx$: int :: 
-    (0 <= idx$) && (idx$ < (R[iir#g] + C[iir#g])) ==> (M[iir#g][idx$ - 0] == AT#RShift(M[iir#c][idx$ - 0], 8))
+  assert {:msg "  Sub-actor action at 14.3 might not preserve the channel invariant (generated #83)"} (forall idx$: int :: 
+    (0 <= idx$) && (idx$ < (R[iir#e] + C[iir#e])) ==> (M[iir#e][idx$] == (171 * M[iir#d][idx$]))
   );
-  assert {:msg "  Sub-actor action at 14.3 might not preserve the channel invariant (generated #65)"} R[iir#c] == (R[iir#g] + C[iir#g]);
-  assert {:msg "  Sub-actor action at 14.3 might not preserve the channel invariant (generated #66)"} (forall idx$: int :: 
-    (0 <= idx$) && (idx$ < (R[iir#d] + C[iir#d])) ==> (M[iir#d][idx$ - 0] == AT#RShift(M[iir#c][idx$ - 0], 8))
+  assert {:msg "  Sub-actor action at 14.3 might not preserve the channel invariant (generated #84)"} (forall idx$: int :: 
+    (0 <= idx$) && (idx$ < (R[iir#d] + C[iir#d])) ==> (M[iir#d][idx$] == AT#RShift(M[iir#c][idx$], 8))
   );
-  assert {:msg "  Sub-actor action at 14.3 might not preserve the channel invariant (generated #67)"} R[iir#c] == (R[iir#d] + C[iir#d]);
-  assert {:msg "  Sub-actor action at 14.3 might not preserve the channel invariant (generated #68)"} (forall idx$: int :: 
-    (0 <= idx$) && (idx$ < (R[iir#e] + C[iir#e])) ==> (M[iir#e][idx$ - 0] == (171 * M[iir#d][idx$ - 0]))
+  assert {:msg "  Sub-actor action at 14.3 might not preserve the channel invariant (generated #85)"} (forall idx$: int :: 
+    (0 <= idx$) && (idx$ < (R[iir#g] + C[iir#g])) ==> (M[iir#g][idx$] == AT#RShift(M[iir#c][idx$], 8))
   );
-  assert {:msg "  Sub-actor action at 14.3 might not preserve the channel invariant (generated #69)"} R[iir#d] == (R[iir#e] + C[iir#e]);
-  assert {:msg "  Sub-actor action at 14.3 might not preserve the channel invariant (generated #70)"} (forall idx$: int :: 
-    (0 <= idx$) && (idx$ < (R[iir#b] + C[iir#b])) ==> (M[iir#b][idx$ - 0] == (85 * M[iir#a][idx$ - 0]))
+  assert {:msg "  Sub-actor action at 14.3 might not preserve the channel invariant (generated #86)"} (forall idx$: int :: 
+    (0 <= idx$) && (idx$ < (R[iir#c] + C[iir#c])) ==> (M[iir#c][idx$] == (M[iir#b][idx$] + M[iir#f][idx$]))
   );
-  assert {:msg "  Sub-actor action at 14.3 might not preserve the channel invariant (generated #71)"} R[iir#a] == (R[iir#b] + C[iir#b]);
-  assert {:msg "  Sub-actor action at 14.3 might not preserve the channel invariant (generated #72)"} (forall idx$: int :: 
-    (0 <= idx$) && (idx$ < ((R[iir#f] + C[iir#f]) - 1)) ==> (M[iir#f][(idx$ + 1) - 0] == M[iir#e][idx$ - 0])
-  );
-  assert {:msg "  Sub-actor action at 14.3 might not preserve the channel invariant (generated #73)"} R[iir#e] == ((R[iir#f] + C[iir#f]) - 1);
-  assert {:msg "  Sub-actor action at 14.3 might not preserve the channel invariant (generated #74)"} R[iir#g] == 0;
-  assert {:msg "  Sub-actor action at 14.3 might not preserve the channel invariant (generated #75)"} 0 <= C[iir#g];
-  assert {:msg "  Sub-actor action at 14.3 might not preserve the channel invariant (generated #76)"} 0 <= R[iir#g];
-  assert {:msg "  Sub-actor action at 14.3 might not preserve the channel invariant (generated #77)"} 0 <= C[iir#f];
-  assert {:msg "  Sub-actor action at 14.3 might not preserve the channel invariant (generated #78)"} 0 <= R[iir#f];
-  assert {:msg "  Sub-actor action at 14.3 might not preserve the channel invariant (generated #79)"} 0 <= C[iir#e];
-  assert {:msg "  Sub-actor action at 14.3 might not preserve the channel invariant (generated #80)"} 0 <= R[iir#e];
-  assert {:msg "  Sub-actor action at 14.3 might not preserve the channel invariant (generated #81)"} 0 <= C[iir#d];
-  assert {:msg "  Sub-actor action at 14.3 might not preserve the channel invariant (generated #82)"} 0 <= R[iir#d];
-  assert {:msg "  Sub-actor action at 14.3 might not preserve the channel invariant (generated #83)"} 0 <= C[iir#c];
-  assert {:msg "  Sub-actor action at 14.3 might not preserve the channel invariant (generated #84)"} 0 <= R[iir#c];
-  assert {:msg "  Sub-actor action at 14.3 might not preserve the channel invariant (generated #85)"} 0 <= C[iir#b];
-  assert {:msg "  Sub-actor action at 14.3 might not preserve the channel invariant (generated #86)"} 0 <= R[iir#b];
-  assert {:msg "  Sub-actor action at 14.3 might not preserve the channel invariant (generated #87)"} (R[iir#a] + C[iir#a]) == C#init[iir#a];
-  assert {:msg "  Sub-actor action at 14.3 might not preserve the channel invariant (generated #88)"} 0 <= C[iir#a];
-  assert {:msg "  Sub-actor action at 14.3 might not preserve the channel invariant (generated #89)"} 0 <= R[iir#a];
   assert {:msg "  28.3: Sub-actor action at 14.3 might not preserve the channel invariant"} (171 * M[iir#g][-1]) == M[iir#f][0];
 }
-procedure iir#anon$5#mulc#anon$3#8()
+procedure iir#anon$5#mulc#anon$3#9()
   modifies C, R, M, St;
 {
   var ActorParam#c: int;
@@ -380,50 +395,47 @@ procedure iir#anon$5#mulc#anon$3#8()
   assume C#init[iir#d] == 0;
   assume C#init[iir#e] == 0;
   assume C#init[iir#g] == 0;
-  assume (forall idx$: int :: 
-    (0 <= idx$) && (idx$ < (R[iir#c] + C[iir#c])) ==> (M[iir#c][idx$ - 0] == (M[iir#b][idx$ - 0] + M[iir#f][idx$ - 0]))
-  );
+  assume 0 <= R[iir#a];
+  assume 0 <= C[iir#a];
+  assume (R[iir#a] + C[iir#a]) == C#init[iir#a];
+  assume 0 <= R[iir#b];
+  assume 0 <= C[iir#b];
+  assume 0 <= R[iir#c];
+  assume 0 <= C[iir#c];
+  assume 0 <= R[iir#d];
+  assume 0 <= C[iir#d];
+  assume 0 <= R[iir#e];
+  assume 0 <= C[iir#e];
+  assume 0 <= R[iir#f];
+  assume 0 <= C[iir#f];
+  assume 0 <= R[iir#g];
+  assume 0 <= C[iir#g];
+  assume R[iir#g] == 0;
+  assume R[iir#e] == ((R[iir#f] + C[iir#f]) - 1);
+  assume R[iir#a] == (R[iir#b] + C[iir#b]);
+  assume R[iir#d] == (R[iir#e] + C[iir#e]);
+  assume R[iir#c] == (R[iir#d] + C[iir#d]);
+  assume R[iir#c] == (R[iir#g] + C[iir#g]);
+  assume R[iir#b] == (R[iir#c] + C[iir#c]);
   assume R[iir#f] == (R[iir#c] + C[iir#c]);
   assume (forall idx$: int :: 
-    (0 <= idx$) && (idx$ < (R[iir#c] + C[iir#c])) ==> (M[iir#c][idx$ - 0] == (M[iir#b][idx$ - 0] + M[iir#f][idx$ - 0]))
+    (1 <= idx$) && (idx$ < (R[iir#f] + C[iir#f])) ==> (M[iir#f][idx$] == M[iir#e][idx$ - 1])
   );
-  assume R[iir#b] == (R[iir#c] + C[iir#c]);
   assume (forall idx$: int :: 
-    (0 <= idx$) && (idx$ < (R[iir#g] + C[iir#g])) ==> (M[iir#g][idx$ - 0] == AT#RShift(M[iir#c][idx$ - 0], 8))
+    (0 <= idx$) && (idx$ < (R[iir#b] + C[iir#b])) ==> (M[iir#b][idx$] == (85 * M[iir#a][idx$]))
   );
-  assume R[iir#c] == (R[iir#g] + C[iir#g]);
   assume (forall idx$: int :: 
-    (0 <= idx$) && (idx$ < (R[iir#d] + C[iir#d])) ==> (M[iir#d][idx$ - 0] == AT#RShift(M[iir#c][idx$ - 0], 8))
+    (0 <= idx$) && (idx$ < (R[iir#e] + C[iir#e])) ==> (M[iir#e][idx$] == (171 * M[iir#d][idx$]))
   );
-  assume R[iir#c] == (R[iir#d] + C[iir#d]);
   assume (forall idx$: int :: 
-    (0 <= idx$) && (idx$ < (R[iir#e] + C[iir#e])) ==> (M[iir#e][idx$ - 0] == (171 * M[iir#d][idx$ - 0]))
+    (0 <= idx$) && (idx$ < (R[iir#d] + C[iir#d])) ==> (M[iir#d][idx$] == AT#RShift(M[iir#c][idx$], 8))
   );
-  assume R[iir#d] == (R[iir#e] + C[iir#e]);
   assume (forall idx$: int :: 
-    (0 <= idx$) && (idx$ < (R[iir#b] + C[iir#b])) ==> (M[iir#b][idx$ - 0] == (85 * M[iir#a][idx$ - 0]))
+    (0 <= idx$) && (idx$ < (R[iir#g] + C[iir#g])) ==> (M[iir#g][idx$] == AT#RShift(M[iir#c][idx$], 8))
   );
-  assume R[iir#a] == (R[iir#b] + C[iir#b]);
   assume (forall idx$: int :: 
-    (0 <= idx$) && (idx$ < ((R[iir#f] + C[iir#f]) - 1)) ==> (M[iir#f][(idx$ + 1) - 0] == M[iir#e][idx$ - 0])
+    (0 <= idx$) && (idx$ < (R[iir#c] + C[iir#c])) ==> (M[iir#c][idx$] == (M[iir#b][idx$] + M[iir#f][idx$]))
   );
-  assume R[iir#e] == ((R[iir#f] + C[iir#f]) - 1);
-  assume R[iir#g] == 0;
-  assume 0 <= C[iir#g];
-  assume 0 <= R[iir#g];
-  assume 0 <= C[iir#f];
-  assume 0 <= R[iir#f];
-  assume 0 <= C[iir#e];
-  assume 0 <= R[iir#e];
-  assume 0 <= C[iir#d];
-  assume 0 <= R[iir#d];
-  assume 0 <= C[iir#c];
-  assume 0 <= R[iir#c];
-  assume 0 <= C[iir#b];
-  assume 0 <= R[iir#b];
-  assume (R[iir#a] + C[iir#a]) == C#init[iir#a];
-  assume 0 <= C[iir#a];
-  assume 0 <= R[iir#a];
   assume (171 * M[iir#g][-1]) == M[iir#f][0];
   assume true;
   assume 1 <= C[iir#d];
@@ -432,53 +444,50 @@ procedure iir#anon$5#mulc#anon$3#8()
   C[iir#d] := C[iir#d] - 1;
   M[iir#e][R[iir#e] + C[iir#e]] := ActorParam#c * in#i;
   C[iir#e] := C[iir#e] + 1;
-  assert {:msg "  Sub-actor action at 14.3 might not preserve the channel invariant (generated #90)"} (forall idx$: int :: 
-    (0 <= idx$) && (idx$ < (R[iir#c] + C[iir#c])) ==> (M[iir#c][idx$ - 0] == (M[iir#b][idx$ - 0] + M[iir#f][idx$ - 0]))
-  );
-  assert {:msg "  Sub-actor action at 14.3 might not preserve the channel invariant (generated #91)"} R[iir#f] == (R[iir#c] + C[iir#c]);
-  assert {:msg "  Sub-actor action at 14.3 might not preserve the channel invariant (generated #92)"} (forall idx$: int :: 
-    (0 <= idx$) && (idx$ < (R[iir#c] + C[iir#c])) ==> (M[iir#c][idx$ - 0] == (M[iir#b][idx$ - 0] + M[iir#f][idx$ - 0]))
-  );
-  assert {:msg "  Sub-actor action at 14.3 might not preserve the channel invariant (generated #93)"} R[iir#b] == (R[iir#c] + C[iir#c]);
-  assert {:msg "  Sub-actor action at 14.3 might not preserve the channel invariant (generated #94)"} (forall idx$: int :: 
-    (0 <= idx$) && (idx$ < (R[iir#g] + C[iir#g])) ==> (M[iir#g][idx$ - 0] == AT#RShift(M[iir#c][idx$ - 0], 8))
-  );
-  assert {:msg "  Sub-actor action at 14.3 might not preserve the channel invariant (generated #95)"} R[iir#c] == (R[iir#g] + C[iir#g]);
-  assert {:msg "  Sub-actor action at 14.3 might not preserve the channel invariant (generated #96)"} (forall idx$: int :: 
-    (0 <= idx$) && (idx$ < (R[iir#d] + C[iir#d])) ==> (M[iir#d][idx$ - 0] == AT#RShift(M[iir#c][idx$ - 0], 8))
-  );
-  assert {:msg "  Sub-actor action at 14.3 might not preserve the channel invariant (generated #97)"} R[iir#c] == (R[iir#d] + C[iir#d]);
-  assert {:msg "  Sub-actor action at 14.3 might not preserve the channel invariant (generated #98)"} (forall idx$: int :: 
-    (0 <= idx$) && (idx$ < (R[iir#e] + C[iir#e])) ==> (M[iir#e][idx$ - 0] == (171 * M[iir#d][idx$ - 0]))
-  );
-  assert {:msg "  Sub-actor action at 14.3 might not preserve the channel invariant (generated #99)"} R[iir#d] == (R[iir#e] + C[iir#e]);
-  assert {:msg "  Sub-actor action at 14.3 might not preserve the channel invariant (generated #100)"} (forall idx$: int :: 
-    (0 <= idx$) && (idx$ < (R[iir#b] + C[iir#b])) ==> (M[iir#b][idx$ - 0] == (85 * M[iir#a][idx$ - 0]))
-  );
-  assert {:msg "  Sub-actor action at 14.3 might not preserve the channel invariant (generated #101)"} R[iir#a] == (R[iir#b] + C[iir#b]);
-  assert {:msg "  Sub-actor action at 14.3 might not preserve the channel invariant (generated #102)"} (forall idx$: int :: 
-    (0 <= idx$) && (idx$ < ((R[iir#f] + C[iir#f]) - 1)) ==> (M[iir#f][(idx$ + 1) - 0] == M[iir#e][idx$ - 0])
-  );
+  assert {:msg "  Sub-actor action at 14.3 might not preserve the channel invariant (generated #87)"} 0 <= R[iir#a];
+  assert {:msg "  Sub-actor action at 14.3 might not preserve the channel invariant (generated #88)"} 0 <= C[iir#a];
+  assert {:msg "  Sub-actor action at 14.3 might not preserve the channel invariant (generated #89)"} (R[iir#a] + C[iir#a]) == C#init[iir#a];
+  assert {:msg "  Sub-actor action at 14.3 might not preserve the channel invariant (generated #90)"} 0 <= R[iir#b];
+  assert {:msg "  Sub-actor action at 14.3 might not preserve the channel invariant (generated #91)"} 0 <= C[iir#b];
+  assert {:msg "  Sub-actor action at 14.3 might not preserve the channel invariant (generated #92)"} 0 <= R[iir#c];
+  assert {:msg "  Sub-actor action at 14.3 might not preserve the channel invariant (generated #93)"} 0 <= C[iir#c];
+  assert {:msg "  Sub-actor action at 14.3 might not preserve the channel invariant (generated #94)"} 0 <= R[iir#d];
+  assert {:msg "  Sub-actor action at 14.3 might not preserve the channel invariant (generated #95)"} 0 <= C[iir#d];
+  assert {:msg "  Sub-actor action at 14.3 might not preserve the channel invariant (generated #96)"} 0 <= R[iir#e];
+  assert {:msg "  Sub-actor action at 14.3 might not preserve the channel invariant (generated #97)"} 0 <= C[iir#e];
+  assert {:msg "  Sub-actor action at 14.3 might not preserve the channel invariant (generated #98)"} 0 <= R[iir#f];
+  assert {:msg "  Sub-actor action at 14.3 might not preserve the channel invariant (generated #99)"} 0 <= C[iir#f];
+  assert {:msg "  Sub-actor action at 14.3 might not preserve the channel invariant (generated #100)"} 0 <= R[iir#g];
+  assert {:msg "  Sub-actor action at 14.3 might not preserve the channel invariant (generated #101)"} 0 <= C[iir#g];
+  assert {:msg "  Sub-actor action at 14.3 might not preserve the channel invariant (generated #102)"} R[iir#g] == 0;
   assert {:msg "  Sub-actor action at 14.3 might not preserve the channel invariant (generated #103)"} R[iir#e] == ((R[iir#f] + C[iir#f]) - 1);
-  assert {:msg "  Sub-actor action at 14.3 might not preserve the channel invariant (generated #104)"} R[iir#g] == 0;
-  assert {:msg "  Sub-actor action at 14.3 might not preserve the channel invariant (generated #105)"} 0 <= C[iir#g];
-  assert {:msg "  Sub-actor action at 14.3 might not preserve the channel invariant (generated #106)"} 0 <= R[iir#g];
-  assert {:msg "  Sub-actor action at 14.3 might not preserve the channel invariant (generated #107)"} 0 <= C[iir#f];
-  assert {:msg "  Sub-actor action at 14.3 might not preserve the channel invariant (generated #108)"} 0 <= R[iir#f];
-  assert {:msg "  Sub-actor action at 14.3 might not preserve the channel invariant (generated #109)"} 0 <= C[iir#e];
-  assert {:msg "  Sub-actor action at 14.3 might not preserve the channel invariant (generated #110)"} 0 <= R[iir#e];
-  assert {:msg "  Sub-actor action at 14.3 might not preserve the channel invariant (generated #111)"} 0 <= C[iir#d];
-  assert {:msg "  Sub-actor action at 14.3 might not preserve the channel invariant (generated #112)"} 0 <= R[iir#d];
-  assert {:msg "  Sub-actor action at 14.3 might not preserve the channel invariant (generated #113)"} 0 <= C[iir#c];
-  assert {:msg "  Sub-actor action at 14.3 might not preserve the channel invariant (generated #114)"} 0 <= R[iir#c];
-  assert {:msg "  Sub-actor action at 14.3 might not preserve the channel invariant (generated #115)"} 0 <= C[iir#b];
-  assert {:msg "  Sub-actor action at 14.3 might not preserve the channel invariant (generated #116)"} 0 <= R[iir#b];
-  assert {:msg "  Sub-actor action at 14.3 might not preserve the channel invariant (generated #117)"} (R[iir#a] + C[iir#a]) == C#init[iir#a];
-  assert {:msg "  Sub-actor action at 14.3 might not preserve the channel invariant (generated #118)"} 0 <= C[iir#a];
-  assert {:msg "  Sub-actor action at 14.3 might not preserve the channel invariant (generated #119)"} 0 <= R[iir#a];
+  assert {:msg "  Sub-actor action at 14.3 might not preserve the channel invariant (generated #104)"} R[iir#a] == (R[iir#b] + C[iir#b]);
+  assert {:msg "  Sub-actor action at 14.3 might not preserve the channel invariant (generated #105)"} R[iir#d] == (R[iir#e] + C[iir#e]);
+  assert {:msg "  Sub-actor action at 14.3 might not preserve the channel invariant (generated #106)"} R[iir#c] == (R[iir#d] + C[iir#d]);
+  assert {:msg "  Sub-actor action at 14.3 might not preserve the channel invariant (generated #107)"} R[iir#c] == (R[iir#g] + C[iir#g]);
+  assert {:msg "  Sub-actor action at 14.3 might not preserve the channel invariant (generated #108)"} R[iir#b] == (R[iir#c] + C[iir#c]);
+  assert {:msg "  Sub-actor action at 14.3 might not preserve the channel invariant (generated #109)"} R[iir#f] == (R[iir#c] + C[iir#c]);
+  assert {:msg "  Sub-actor action at 14.3 might not preserve the channel invariant (generated #110)"} (forall idx$: int :: 
+    (1 <= idx$) && (idx$ < (R[iir#f] + C[iir#f])) ==> (M[iir#f][idx$] == M[iir#e][idx$ - 1])
+  );
+  assert {:msg "  Sub-actor action at 14.3 might not preserve the channel invariant (generated #111)"} (forall idx$: int :: 
+    (0 <= idx$) && (idx$ < (R[iir#b] + C[iir#b])) ==> (M[iir#b][idx$] == (85 * M[iir#a][idx$]))
+  );
+  assert {:msg "  Sub-actor action at 14.3 might not preserve the channel invariant (generated #112)"} (forall idx$: int :: 
+    (0 <= idx$) && (idx$ < (R[iir#e] + C[iir#e])) ==> (M[iir#e][idx$] == (171 * M[iir#d][idx$]))
+  );
+  assert {:msg "  Sub-actor action at 14.3 might not preserve the channel invariant (generated #113)"} (forall idx$: int :: 
+    (0 <= idx$) && (idx$ < (R[iir#d] + C[iir#d])) ==> (M[iir#d][idx$] == AT#RShift(M[iir#c][idx$], 8))
+  );
+  assert {:msg "  Sub-actor action at 14.3 might not preserve the channel invariant (generated #114)"} (forall idx$: int :: 
+    (0 <= idx$) && (idx$ < (R[iir#g] + C[iir#g])) ==> (M[iir#g][idx$] == AT#RShift(M[iir#c][idx$], 8))
+  );
+  assert {:msg "  Sub-actor action at 14.3 might not preserve the channel invariant (generated #115)"} (forall idx$: int :: 
+    (0 <= idx$) && (idx$ < (R[iir#c] + C[iir#c])) ==> (M[iir#c][idx$] == (M[iir#b][idx$] + M[iir#f][idx$]))
+  );
   assert {:msg "  28.3: Sub-actor action at 14.3 might not preserve the channel invariant"} (171 * M[iir#g][-1]) == M[iir#f][0];
 }
-procedure iir#anon$5#rshift#anon$4#9()
+procedure iir#anon$5#rshift#anon$4#10()
   modifies C, R, M, St;
 {
   var ActorParam#s: int;
@@ -491,50 +500,47 @@ procedure iir#anon$5#rshift#anon$4#9()
   assume C#init[iir#d] == 0;
   assume C#init[iir#e] == 0;
   assume C#init[iir#g] == 0;
-  assume (forall idx$: int :: 
-    (0 <= idx$) && (idx$ < (R[iir#c] + C[iir#c])) ==> (M[iir#c][idx$ - 0] == (M[iir#b][idx$ - 0] + M[iir#f][idx$ - 0]))
-  );
+  assume 0 <= R[iir#a];
+  assume 0 <= C[iir#a];
+  assume (R[iir#a] + C[iir#a]) == C#init[iir#a];
+  assume 0 <= R[iir#b];
+  assume 0 <= C[iir#b];
+  assume 0 <= R[iir#c];
+  assume 0 <= C[iir#c];
+  assume 0 <= R[iir#d];
+  assume 0 <= C[iir#d];
+  assume 0 <= R[iir#e];
+  assume 0 <= C[iir#e];
+  assume 0 <= R[iir#f];
+  assume 0 <= C[iir#f];
+  assume 0 <= R[iir#g];
+  assume 0 <= C[iir#g];
+  assume R[iir#g] == 0;
+  assume R[iir#e] == ((R[iir#f] + C[iir#f]) - 1);
+  assume R[iir#a] == (R[iir#b] + C[iir#b]);
+  assume R[iir#d] == (R[iir#e] + C[iir#e]);
+  assume R[iir#c] == (R[iir#d] + C[iir#d]);
+  assume R[iir#c] == (R[iir#g] + C[iir#g]);
+  assume R[iir#b] == (R[iir#c] + C[iir#c]);
   assume R[iir#f] == (R[iir#c] + C[iir#c]);
   assume (forall idx$: int :: 
-    (0 <= idx$) && (idx$ < (R[iir#c] + C[iir#c])) ==> (M[iir#c][idx$ - 0] == (M[iir#b][idx$ - 0] + M[iir#f][idx$ - 0]))
+    (1 <= idx$) && (idx$ < (R[iir#f] + C[iir#f])) ==> (M[iir#f][idx$] == M[iir#e][idx$ - 1])
   );
-  assume R[iir#b] == (R[iir#c] + C[iir#c]);
   assume (forall idx$: int :: 
-    (0 <= idx$) && (idx$ < (R[iir#g] + C[iir#g])) ==> (M[iir#g][idx$ - 0] == AT#RShift(M[iir#c][idx$ - 0], 8))
+    (0 <= idx$) && (idx$ < (R[iir#b] + C[iir#b])) ==> (M[iir#b][idx$] == (85 * M[iir#a][idx$]))
   );
-  assume R[iir#c] == (R[iir#g] + C[iir#g]);
   assume (forall idx$: int :: 
-    (0 <= idx$) && (idx$ < (R[iir#d] + C[iir#d])) ==> (M[iir#d][idx$ - 0] == AT#RShift(M[iir#c][idx$ - 0], 8))
+    (0 <= idx$) && (idx$ < (R[iir#e] + C[iir#e])) ==> (M[iir#e][idx$] == (171 * M[iir#d][idx$]))
   );
-  assume R[iir#c] == (R[iir#d] + C[iir#d]);
   assume (forall idx$: int :: 
-    (0 <= idx$) && (idx$ < (R[iir#e] + C[iir#e])) ==> (M[iir#e][idx$ - 0] == (171 * M[iir#d][idx$ - 0]))
+    (0 <= idx$) && (idx$ < (R[iir#d] + C[iir#d])) ==> (M[iir#d][idx$] == AT#RShift(M[iir#c][idx$], 8))
   );
-  assume R[iir#d] == (R[iir#e] + C[iir#e]);
   assume (forall idx$: int :: 
-    (0 <= idx$) && (idx$ < (R[iir#b] + C[iir#b])) ==> (M[iir#b][idx$ - 0] == (85 * M[iir#a][idx$ - 0]))
+    (0 <= idx$) && (idx$ < (R[iir#g] + C[iir#g])) ==> (M[iir#g][idx$] == AT#RShift(M[iir#c][idx$], 8))
   );
-  assume R[iir#a] == (R[iir#b] + C[iir#b]);
   assume (forall idx$: int :: 
-    (0 <= idx$) && (idx$ < ((R[iir#f] + C[iir#f]) - 1)) ==> (M[iir#f][(idx$ + 1) - 0] == M[iir#e][idx$ - 0])
+    (0 <= idx$) && (idx$ < (R[iir#c] + C[iir#c])) ==> (M[iir#c][idx$] == (M[iir#b][idx$] + M[iir#f][idx$]))
   );
-  assume R[iir#e] == ((R[iir#f] + C[iir#f]) - 1);
-  assume R[iir#g] == 0;
-  assume 0 <= C[iir#g];
-  assume 0 <= R[iir#g];
-  assume 0 <= C[iir#f];
-  assume 0 <= R[iir#f];
-  assume 0 <= C[iir#e];
-  assume 0 <= R[iir#e];
-  assume 0 <= C[iir#d];
-  assume 0 <= R[iir#d];
-  assume 0 <= C[iir#c];
-  assume 0 <= R[iir#c];
-  assume 0 <= C[iir#b];
-  assume 0 <= R[iir#b];
-  assume (R[iir#a] + C[iir#a]) == C#init[iir#a];
-  assume 0 <= C[iir#a];
-  assume 0 <= R[iir#a];
   assume (171 * M[iir#g][-1]) == M[iir#f][0];
   assume true;
   assume 1 <= C[iir#c];
@@ -545,53 +551,50 @@ procedure iir#anon$5#rshift#anon$4#9()
   C[iir#d] := C[iir#d] + 1;
   M[iir#g][R[iir#g] + C[iir#g]] := AT#RShift(in#i, ActorParam#s);
   C[iir#g] := C[iir#g] + 1;
-  assert {:msg "  Sub-actor action at 19.3 might not preserve the channel invariant (generated #120)"} (forall idx$: int :: 
-    (0 <= idx$) && (idx$ < (R[iir#c] + C[iir#c])) ==> (M[iir#c][idx$ - 0] == (M[iir#b][idx$ - 0] + M[iir#f][idx$ - 0]))
+  assert {:msg "  Sub-actor action at 19.3 might not preserve the channel invariant (generated #116)"} 0 <= R[iir#a];
+  assert {:msg "  Sub-actor action at 19.3 might not preserve the channel invariant (generated #117)"} 0 <= C[iir#a];
+  assert {:msg "  Sub-actor action at 19.3 might not preserve the channel invariant (generated #118)"} (R[iir#a] + C[iir#a]) == C#init[iir#a];
+  assert {:msg "  Sub-actor action at 19.3 might not preserve the channel invariant (generated #119)"} 0 <= R[iir#b];
+  assert {:msg "  Sub-actor action at 19.3 might not preserve the channel invariant (generated #120)"} 0 <= C[iir#b];
+  assert {:msg "  Sub-actor action at 19.3 might not preserve the channel invariant (generated #121)"} 0 <= R[iir#c];
+  assert {:msg "  Sub-actor action at 19.3 might not preserve the channel invariant (generated #122)"} 0 <= C[iir#c];
+  assert {:msg "  Sub-actor action at 19.3 might not preserve the channel invariant (generated #123)"} 0 <= R[iir#d];
+  assert {:msg "  Sub-actor action at 19.3 might not preserve the channel invariant (generated #124)"} 0 <= C[iir#d];
+  assert {:msg "  Sub-actor action at 19.3 might not preserve the channel invariant (generated #125)"} 0 <= R[iir#e];
+  assert {:msg "  Sub-actor action at 19.3 might not preserve the channel invariant (generated #126)"} 0 <= C[iir#e];
+  assert {:msg "  Sub-actor action at 19.3 might not preserve the channel invariant (generated #127)"} 0 <= R[iir#f];
+  assert {:msg "  Sub-actor action at 19.3 might not preserve the channel invariant (generated #128)"} 0 <= C[iir#f];
+  assert {:msg "  Sub-actor action at 19.3 might not preserve the channel invariant (generated #129)"} 0 <= R[iir#g];
+  assert {:msg "  Sub-actor action at 19.3 might not preserve the channel invariant (generated #130)"} 0 <= C[iir#g];
+  assert {:msg "  Sub-actor action at 19.3 might not preserve the channel invariant (generated #131)"} R[iir#g] == 0;
+  assert {:msg "  Sub-actor action at 19.3 might not preserve the channel invariant (generated #132)"} R[iir#e] == ((R[iir#f] + C[iir#f]) - 1);
+  assert {:msg "  Sub-actor action at 19.3 might not preserve the channel invariant (generated #133)"} R[iir#a] == (R[iir#b] + C[iir#b]);
+  assert {:msg "  Sub-actor action at 19.3 might not preserve the channel invariant (generated #134)"} R[iir#d] == (R[iir#e] + C[iir#e]);
+  assert {:msg "  Sub-actor action at 19.3 might not preserve the channel invariant (generated #135)"} R[iir#c] == (R[iir#d] + C[iir#d]);
+  assert {:msg "  Sub-actor action at 19.3 might not preserve the channel invariant (generated #136)"} R[iir#c] == (R[iir#g] + C[iir#g]);
+  assert {:msg "  Sub-actor action at 19.3 might not preserve the channel invariant (generated #137)"} R[iir#b] == (R[iir#c] + C[iir#c]);
+  assert {:msg "  Sub-actor action at 19.3 might not preserve the channel invariant (generated #138)"} R[iir#f] == (R[iir#c] + C[iir#c]);
+  assert {:msg "  Sub-actor action at 19.3 might not preserve the channel invariant (generated #139)"} (forall idx$: int :: 
+    (1 <= idx$) && (idx$ < (R[iir#f] + C[iir#f])) ==> (M[iir#f][idx$] == M[iir#e][idx$ - 1])
   );
-  assert {:msg "  Sub-actor action at 19.3 might not preserve the channel invariant (generated #121)"} R[iir#f] == (R[iir#c] + C[iir#c]);
-  assert {:msg "  Sub-actor action at 19.3 might not preserve the channel invariant (generated #122)"} (forall idx$: int :: 
-    (0 <= idx$) && (idx$ < (R[iir#c] + C[iir#c])) ==> (M[iir#c][idx$ - 0] == (M[iir#b][idx$ - 0] + M[iir#f][idx$ - 0]))
+  assert {:msg "  Sub-actor action at 19.3 might not preserve the channel invariant (generated #140)"} (forall idx$: int :: 
+    (0 <= idx$) && (idx$ < (R[iir#b] + C[iir#b])) ==> (M[iir#b][idx$] == (85 * M[iir#a][idx$]))
   );
-  assert {:msg "  Sub-actor action at 19.3 might not preserve the channel invariant (generated #123)"} R[iir#b] == (R[iir#c] + C[iir#c]);
-  assert {:msg "  Sub-actor action at 19.3 might not preserve the channel invariant (generated #124)"} (forall idx$: int :: 
-    (0 <= idx$) && (idx$ < (R[iir#g] + C[iir#g])) ==> (M[iir#g][idx$ - 0] == AT#RShift(M[iir#c][idx$ - 0], 8))
+  assert {:msg "  Sub-actor action at 19.3 might not preserve the channel invariant (generated #141)"} (forall idx$: int :: 
+    (0 <= idx$) && (idx$ < (R[iir#e] + C[iir#e])) ==> (M[iir#e][idx$] == (171 * M[iir#d][idx$]))
   );
-  assert {:msg "  Sub-actor action at 19.3 might not preserve the channel invariant (generated #125)"} R[iir#c] == (R[iir#g] + C[iir#g]);
-  assert {:msg "  Sub-actor action at 19.3 might not preserve the channel invariant (generated #126)"} (forall idx$: int :: 
-    (0 <= idx$) && (idx$ < (R[iir#d] + C[iir#d])) ==> (M[iir#d][idx$ - 0] == AT#RShift(M[iir#c][idx$ - 0], 8))
+  assert {:msg "  Sub-actor action at 19.3 might not preserve the channel invariant (generated #142)"} (forall idx$: int :: 
+    (0 <= idx$) && (idx$ < (R[iir#d] + C[iir#d])) ==> (M[iir#d][idx$] == AT#RShift(M[iir#c][idx$], 8))
   );
-  assert {:msg "  Sub-actor action at 19.3 might not preserve the channel invariant (generated #127)"} R[iir#c] == (R[iir#d] + C[iir#d]);
-  assert {:msg "  Sub-actor action at 19.3 might not preserve the channel invariant (generated #128)"} (forall idx$: int :: 
-    (0 <= idx$) && (idx$ < (R[iir#e] + C[iir#e])) ==> (M[iir#e][idx$ - 0] == (171 * M[iir#d][idx$ - 0]))
+  assert {:msg "  Sub-actor action at 19.3 might not preserve the channel invariant (generated #143)"} (forall idx$: int :: 
+    (0 <= idx$) && (idx$ < (R[iir#g] + C[iir#g])) ==> (M[iir#g][idx$] == AT#RShift(M[iir#c][idx$], 8))
   );
-  assert {:msg "  Sub-actor action at 19.3 might not preserve the channel invariant (generated #129)"} R[iir#d] == (R[iir#e] + C[iir#e]);
-  assert {:msg "  Sub-actor action at 19.3 might not preserve the channel invariant (generated #130)"} (forall idx$: int :: 
-    (0 <= idx$) && (idx$ < (R[iir#b] + C[iir#b])) ==> (M[iir#b][idx$ - 0] == (85 * M[iir#a][idx$ - 0]))
+  assert {:msg "  Sub-actor action at 19.3 might not preserve the channel invariant (generated #144)"} (forall idx$: int :: 
+    (0 <= idx$) && (idx$ < (R[iir#c] + C[iir#c])) ==> (M[iir#c][idx$] == (M[iir#b][idx$] + M[iir#f][idx$]))
   );
-  assert {:msg "  Sub-actor action at 19.3 might not preserve the channel invariant (generated #131)"} R[iir#a] == (R[iir#b] + C[iir#b]);
-  assert {:msg "  Sub-actor action at 19.3 might not preserve the channel invariant (generated #132)"} (forall idx$: int :: 
-    (0 <= idx$) && (idx$ < ((R[iir#f] + C[iir#f]) - 1)) ==> (M[iir#f][(idx$ + 1) - 0] == M[iir#e][idx$ - 0])
-  );
-  assert {:msg "  Sub-actor action at 19.3 might not preserve the channel invariant (generated #133)"} R[iir#e] == ((R[iir#f] + C[iir#f]) - 1);
-  assert {:msg "  Sub-actor action at 19.3 might not preserve the channel invariant (generated #134)"} R[iir#g] == 0;
-  assert {:msg "  Sub-actor action at 19.3 might not preserve the channel invariant (generated #135)"} 0 <= C[iir#g];
-  assert {:msg "  Sub-actor action at 19.3 might not preserve the channel invariant (generated #136)"} 0 <= R[iir#g];
-  assert {:msg "  Sub-actor action at 19.3 might not preserve the channel invariant (generated #137)"} 0 <= C[iir#f];
-  assert {:msg "  Sub-actor action at 19.3 might not preserve the channel invariant (generated #138)"} 0 <= R[iir#f];
-  assert {:msg "  Sub-actor action at 19.3 might not preserve the channel invariant (generated #139)"} 0 <= C[iir#e];
-  assert {:msg "  Sub-actor action at 19.3 might not preserve the channel invariant (generated #140)"} 0 <= R[iir#e];
-  assert {:msg "  Sub-actor action at 19.3 might not preserve the channel invariant (generated #141)"} 0 <= C[iir#d];
-  assert {:msg "  Sub-actor action at 19.3 might not preserve the channel invariant (generated #142)"} 0 <= R[iir#d];
-  assert {:msg "  Sub-actor action at 19.3 might not preserve the channel invariant (generated #143)"} 0 <= C[iir#c];
-  assert {:msg "  Sub-actor action at 19.3 might not preserve the channel invariant (generated #144)"} 0 <= R[iir#c];
-  assert {:msg "  Sub-actor action at 19.3 might not preserve the channel invariant (generated #145)"} 0 <= C[iir#b];
-  assert {:msg "  Sub-actor action at 19.3 might not preserve the channel invariant (generated #146)"} 0 <= R[iir#b];
-  assert {:msg "  Sub-actor action at 19.3 might not preserve the channel invariant (generated #147)"} (R[iir#a] + C[iir#a]) == C#init[iir#a];
-  assert {:msg "  Sub-actor action at 19.3 might not preserve the channel invariant (generated #148)"} 0 <= C[iir#a];
-  assert {:msg "  Sub-actor action at 19.3 might not preserve the channel invariant (generated #149)"} 0 <= R[iir#a];
   assert {:msg "  28.3: Sub-actor action at 19.3 might not preserve the channel invariant"} (171 * M[iir#g][-1]) == M[iir#f][0];
 }
-procedure iir#anon$5#add#anon$0#10()
+procedure iir#anon$5#add#anon$0#11()
   modifies C, R, M, St;
 {
   var St#next: State;
@@ -603,50 +606,47 @@ procedure iir#anon$5#add#anon$0#10()
   assume C#init[iir#d] == 0;
   assume C#init[iir#e] == 0;
   assume C#init[iir#g] == 0;
-  assume (forall idx$: int :: 
-    (0 <= idx$) && (idx$ < (R[iir#c] + C[iir#c])) ==> (M[iir#c][idx$ - 0] == (M[iir#b][idx$ - 0] + M[iir#f][idx$ - 0]))
-  );
+  assume 0 <= R[iir#a];
+  assume 0 <= C[iir#a];
+  assume (R[iir#a] + C[iir#a]) == C#init[iir#a];
+  assume 0 <= R[iir#b];
+  assume 0 <= C[iir#b];
+  assume 0 <= R[iir#c];
+  assume 0 <= C[iir#c];
+  assume 0 <= R[iir#d];
+  assume 0 <= C[iir#d];
+  assume 0 <= R[iir#e];
+  assume 0 <= C[iir#e];
+  assume 0 <= R[iir#f];
+  assume 0 <= C[iir#f];
+  assume 0 <= R[iir#g];
+  assume 0 <= C[iir#g];
+  assume R[iir#g] == 0;
+  assume R[iir#e] == ((R[iir#f] + C[iir#f]) - 1);
+  assume R[iir#a] == (R[iir#b] + C[iir#b]);
+  assume R[iir#d] == (R[iir#e] + C[iir#e]);
+  assume R[iir#c] == (R[iir#d] + C[iir#d]);
+  assume R[iir#c] == (R[iir#g] + C[iir#g]);
+  assume R[iir#b] == (R[iir#c] + C[iir#c]);
   assume R[iir#f] == (R[iir#c] + C[iir#c]);
   assume (forall idx$: int :: 
-    (0 <= idx$) && (idx$ < (R[iir#c] + C[iir#c])) ==> (M[iir#c][idx$ - 0] == (M[iir#b][idx$ - 0] + M[iir#f][idx$ - 0]))
+    (1 <= idx$) && (idx$ < (R[iir#f] + C[iir#f])) ==> (M[iir#f][idx$] == M[iir#e][idx$ - 1])
   );
-  assume R[iir#b] == (R[iir#c] + C[iir#c]);
   assume (forall idx$: int :: 
-    (0 <= idx$) && (idx$ < (R[iir#g] + C[iir#g])) ==> (M[iir#g][idx$ - 0] == AT#RShift(M[iir#c][idx$ - 0], 8))
+    (0 <= idx$) && (idx$ < (R[iir#b] + C[iir#b])) ==> (M[iir#b][idx$] == (85 * M[iir#a][idx$]))
   );
-  assume R[iir#c] == (R[iir#g] + C[iir#g]);
   assume (forall idx$: int :: 
-    (0 <= idx$) && (idx$ < (R[iir#d] + C[iir#d])) ==> (M[iir#d][idx$ - 0] == AT#RShift(M[iir#c][idx$ - 0], 8))
+    (0 <= idx$) && (idx$ < (R[iir#e] + C[iir#e])) ==> (M[iir#e][idx$] == (171 * M[iir#d][idx$]))
   );
-  assume R[iir#c] == (R[iir#d] + C[iir#d]);
   assume (forall idx$: int :: 
-    (0 <= idx$) && (idx$ < (R[iir#e] + C[iir#e])) ==> (M[iir#e][idx$ - 0] == (171 * M[iir#d][idx$ - 0]))
+    (0 <= idx$) && (idx$ < (R[iir#d] + C[iir#d])) ==> (M[iir#d][idx$] == AT#RShift(M[iir#c][idx$], 8))
   );
-  assume R[iir#d] == (R[iir#e] + C[iir#e]);
   assume (forall idx$: int :: 
-    (0 <= idx$) && (idx$ < (R[iir#b] + C[iir#b])) ==> (M[iir#b][idx$ - 0] == (85 * M[iir#a][idx$ - 0]))
+    (0 <= idx$) && (idx$ < (R[iir#g] + C[iir#g])) ==> (M[iir#g][idx$] == AT#RShift(M[iir#c][idx$], 8))
   );
-  assume R[iir#a] == (R[iir#b] + C[iir#b]);
   assume (forall idx$: int :: 
-    (0 <= idx$) && (idx$ < ((R[iir#f] + C[iir#f]) - 1)) ==> (M[iir#f][(idx$ + 1) - 0] == M[iir#e][idx$ - 0])
+    (0 <= idx$) && (idx$ < (R[iir#c] + C[iir#c])) ==> (M[iir#c][idx$] == (M[iir#b][idx$] + M[iir#f][idx$]))
   );
-  assume R[iir#e] == ((R[iir#f] + C[iir#f]) - 1);
-  assume R[iir#g] == 0;
-  assume 0 <= C[iir#g];
-  assume 0 <= R[iir#g];
-  assume 0 <= C[iir#f];
-  assume 0 <= R[iir#f];
-  assume 0 <= C[iir#e];
-  assume 0 <= R[iir#e];
-  assume 0 <= C[iir#d];
-  assume 0 <= R[iir#d];
-  assume 0 <= C[iir#c];
-  assume 0 <= R[iir#c];
-  assume 0 <= C[iir#b];
-  assume 0 <= R[iir#b];
-  assume (R[iir#a] + C[iir#a]) == C#init[iir#a];
-  assume 0 <= C[iir#a];
-  assume 0 <= R[iir#a];
   assume (171 * M[iir#g][-1]) == M[iir#f][0];
   assume true;
   assume (1 <= C[iir#b]) && (1 <= C[iir#f]);
@@ -658,53 +658,50 @@ procedure iir#anon$5#add#anon$0#10()
   C[iir#f] := C[iir#f] - 1;
   M[iir#c][R[iir#c] + C[iir#c]] := in1#i + in2#j;
   C[iir#c] := C[iir#c] + 1;
-  assert {:msg "  Sub-actor action at 3.3 might not preserve the channel invariant (generated #150)"} (forall idx$: int :: 
-    (0 <= idx$) && (idx$ < (R[iir#c] + C[iir#c])) ==> (M[iir#c][idx$ - 0] == (M[iir#b][idx$ - 0] + M[iir#f][idx$ - 0]))
+  assert {:msg "  Sub-actor action at 3.3 might not preserve the channel invariant (generated #145)"} 0 <= R[iir#a];
+  assert {:msg "  Sub-actor action at 3.3 might not preserve the channel invariant (generated #146)"} 0 <= C[iir#a];
+  assert {:msg "  Sub-actor action at 3.3 might not preserve the channel invariant (generated #147)"} (R[iir#a] + C[iir#a]) == C#init[iir#a];
+  assert {:msg "  Sub-actor action at 3.3 might not preserve the channel invariant (generated #148)"} 0 <= R[iir#b];
+  assert {:msg "  Sub-actor action at 3.3 might not preserve the channel invariant (generated #149)"} 0 <= C[iir#b];
+  assert {:msg "  Sub-actor action at 3.3 might not preserve the channel invariant (generated #150)"} 0 <= R[iir#c];
+  assert {:msg "  Sub-actor action at 3.3 might not preserve the channel invariant (generated #151)"} 0 <= C[iir#c];
+  assert {:msg "  Sub-actor action at 3.3 might not preserve the channel invariant (generated #152)"} 0 <= R[iir#d];
+  assert {:msg "  Sub-actor action at 3.3 might not preserve the channel invariant (generated #153)"} 0 <= C[iir#d];
+  assert {:msg "  Sub-actor action at 3.3 might not preserve the channel invariant (generated #154)"} 0 <= R[iir#e];
+  assert {:msg "  Sub-actor action at 3.3 might not preserve the channel invariant (generated #155)"} 0 <= C[iir#e];
+  assert {:msg "  Sub-actor action at 3.3 might not preserve the channel invariant (generated #156)"} 0 <= R[iir#f];
+  assert {:msg "  Sub-actor action at 3.3 might not preserve the channel invariant (generated #157)"} 0 <= C[iir#f];
+  assert {:msg "  Sub-actor action at 3.3 might not preserve the channel invariant (generated #158)"} 0 <= R[iir#g];
+  assert {:msg "  Sub-actor action at 3.3 might not preserve the channel invariant (generated #159)"} 0 <= C[iir#g];
+  assert {:msg "  Sub-actor action at 3.3 might not preserve the channel invariant (generated #160)"} R[iir#g] == 0;
+  assert {:msg "  Sub-actor action at 3.3 might not preserve the channel invariant (generated #161)"} R[iir#e] == ((R[iir#f] + C[iir#f]) - 1);
+  assert {:msg "  Sub-actor action at 3.3 might not preserve the channel invariant (generated #162)"} R[iir#a] == (R[iir#b] + C[iir#b]);
+  assert {:msg "  Sub-actor action at 3.3 might not preserve the channel invariant (generated #163)"} R[iir#d] == (R[iir#e] + C[iir#e]);
+  assert {:msg "  Sub-actor action at 3.3 might not preserve the channel invariant (generated #164)"} R[iir#c] == (R[iir#d] + C[iir#d]);
+  assert {:msg "  Sub-actor action at 3.3 might not preserve the channel invariant (generated #165)"} R[iir#c] == (R[iir#g] + C[iir#g]);
+  assert {:msg "  Sub-actor action at 3.3 might not preserve the channel invariant (generated #166)"} R[iir#b] == (R[iir#c] + C[iir#c]);
+  assert {:msg "  Sub-actor action at 3.3 might not preserve the channel invariant (generated #167)"} R[iir#f] == (R[iir#c] + C[iir#c]);
+  assert {:msg "  Sub-actor action at 3.3 might not preserve the channel invariant (generated #168)"} (forall idx$: int :: 
+    (1 <= idx$) && (idx$ < (R[iir#f] + C[iir#f])) ==> (M[iir#f][idx$] == M[iir#e][idx$ - 1])
   );
-  assert {:msg "  Sub-actor action at 3.3 might not preserve the channel invariant (generated #151)"} R[iir#f] == (R[iir#c] + C[iir#c]);
-  assert {:msg "  Sub-actor action at 3.3 might not preserve the channel invariant (generated #152)"} (forall idx$: int :: 
-    (0 <= idx$) && (idx$ < (R[iir#c] + C[iir#c])) ==> (M[iir#c][idx$ - 0] == (M[iir#b][idx$ - 0] + M[iir#f][idx$ - 0]))
+  assert {:msg "  Sub-actor action at 3.3 might not preserve the channel invariant (generated #169)"} (forall idx$: int :: 
+    (0 <= idx$) && (idx$ < (R[iir#b] + C[iir#b])) ==> (M[iir#b][idx$] == (85 * M[iir#a][idx$]))
   );
-  assert {:msg "  Sub-actor action at 3.3 might not preserve the channel invariant (generated #153)"} R[iir#b] == (R[iir#c] + C[iir#c]);
-  assert {:msg "  Sub-actor action at 3.3 might not preserve the channel invariant (generated #154)"} (forall idx$: int :: 
-    (0 <= idx$) && (idx$ < (R[iir#g] + C[iir#g])) ==> (M[iir#g][idx$ - 0] == AT#RShift(M[iir#c][idx$ - 0], 8))
+  assert {:msg "  Sub-actor action at 3.3 might not preserve the channel invariant (generated #170)"} (forall idx$: int :: 
+    (0 <= idx$) && (idx$ < (R[iir#e] + C[iir#e])) ==> (M[iir#e][idx$] == (171 * M[iir#d][idx$]))
   );
-  assert {:msg "  Sub-actor action at 3.3 might not preserve the channel invariant (generated #155)"} R[iir#c] == (R[iir#g] + C[iir#g]);
-  assert {:msg "  Sub-actor action at 3.3 might not preserve the channel invariant (generated #156)"} (forall idx$: int :: 
-    (0 <= idx$) && (idx$ < (R[iir#d] + C[iir#d])) ==> (M[iir#d][idx$ - 0] == AT#RShift(M[iir#c][idx$ - 0], 8))
+  assert {:msg "  Sub-actor action at 3.3 might not preserve the channel invariant (generated #171)"} (forall idx$: int :: 
+    (0 <= idx$) && (idx$ < (R[iir#d] + C[iir#d])) ==> (M[iir#d][idx$] == AT#RShift(M[iir#c][idx$], 8))
   );
-  assert {:msg "  Sub-actor action at 3.3 might not preserve the channel invariant (generated #157)"} R[iir#c] == (R[iir#d] + C[iir#d]);
-  assert {:msg "  Sub-actor action at 3.3 might not preserve the channel invariant (generated #158)"} (forall idx$: int :: 
-    (0 <= idx$) && (idx$ < (R[iir#e] + C[iir#e])) ==> (M[iir#e][idx$ - 0] == (171 * M[iir#d][idx$ - 0]))
+  assert {:msg "  Sub-actor action at 3.3 might not preserve the channel invariant (generated #172)"} (forall idx$: int :: 
+    (0 <= idx$) && (idx$ < (R[iir#g] + C[iir#g])) ==> (M[iir#g][idx$] == AT#RShift(M[iir#c][idx$], 8))
   );
-  assert {:msg "  Sub-actor action at 3.3 might not preserve the channel invariant (generated #159)"} R[iir#d] == (R[iir#e] + C[iir#e]);
-  assert {:msg "  Sub-actor action at 3.3 might not preserve the channel invariant (generated #160)"} (forall idx$: int :: 
-    (0 <= idx$) && (idx$ < (R[iir#b] + C[iir#b])) ==> (M[iir#b][idx$ - 0] == (85 * M[iir#a][idx$ - 0]))
+  assert {:msg "  Sub-actor action at 3.3 might not preserve the channel invariant (generated #173)"} (forall idx$: int :: 
+    (0 <= idx$) && (idx$ < (R[iir#c] + C[iir#c])) ==> (M[iir#c][idx$] == (M[iir#b][idx$] + M[iir#f][idx$]))
   );
-  assert {:msg "  Sub-actor action at 3.3 might not preserve the channel invariant (generated #161)"} R[iir#a] == (R[iir#b] + C[iir#b]);
-  assert {:msg "  Sub-actor action at 3.3 might not preserve the channel invariant (generated #162)"} (forall idx$: int :: 
-    (0 <= idx$) && (idx$ < ((R[iir#f] + C[iir#f]) - 1)) ==> (M[iir#f][(idx$ + 1) - 0] == M[iir#e][idx$ - 0])
-  );
-  assert {:msg "  Sub-actor action at 3.3 might not preserve the channel invariant (generated #163)"} R[iir#e] == ((R[iir#f] + C[iir#f]) - 1);
-  assert {:msg "  Sub-actor action at 3.3 might not preserve the channel invariant (generated #164)"} R[iir#g] == 0;
-  assert {:msg "  Sub-actor action at 3.3 might not preserve the channel invariant (generated #165)"} 0 <= C[iir#g];
-  assert {:msg "  Sub-actor action at 3.3 might not preserve the channel invariant (generated #166)"} 0 <= R[iir#g];
-  assert {:msg "  Sub-actor action at 3.3 might not preserve the channel invariant (generated #167)"} 0 <= C[iir#f];
-  assert {:msg "  Sub-actor action at 3.3 might not preserve the channel invariant (generated #168)"} 0 <= R[iir#f];
-  assert {:msg "  Sub-actor action at 3.3 might not preserve the channel invariant (generated #169)"} 0 <= C[iir#e];
-  assert {:msg "  Sub-actor action at 3.3 might not preserve the channel invariant (generated #170)"} 0 <= R[iir#e];
-  assert {:msg "  Sub-actor action at 3.3 might not preserve the channel invariant (generated #171)"} 0 <= C[iir#d];
-  assert {:msg "  Sub-actor action at 3.3 might not preserve the channel invariant (generated #172)"} 0 <= R[iir#d];
-  assert {:msg "  Sub-actor action at 3.3 might not preserve the channel invariant (generated #173)"} 0 <= C[iir#c];
-  assert {:msg "  Sub-actor action at 3.3 might not preserve the channel invariant (generated #174)"} 0 <= R[iir#c];
-  assert {:msg "  Sub-actor action at 3.3 might not preserve the channel invariant (generated #175)"} 0 <= C[iir#b];
-  assert {:msg "  Sub-actor action at 3.3 might not preserve the channel invariant (generated #176)"} 0 <= R[iir#b];
-  assert {:msg "  Sub-actor action at 3.3 might not preserve the channel invariant (generated #177)"} (R[iir#a] + C[iir#a]) == C#init[iir#a];
-  assert {:msg "  Sub-actor action at 3.3 might not preserve the channel invariant (generated #178)"} 0 <= C[iir#a];
-  assert {:msg "  Sub-actor action at 3.3 might not preserve the channel invariant (generated #179)"} 0 <= R[iir#a];
   assert {:msg "  28.3: Sub-actor action at 3.3 might not preserve the channel invariant"} (171 * M[iir#g][-1]) == M[iir#f][0];
 }
-procedure iir#anon$5#exit#11()
+procedure iir#anon$5#exit#12()
   modifies C, R, M, St;
 {
   assume C#init[iir#a] == 1;
@@ -713,50 +710,47 @@ procedure iir#anon$5#exit#11()
   assume C#init[iir#d] == 0;
   assume C#init[iir#e] == 0;
   assume C#init[iir#g] == 0;
-  assume (forall idx$: int :: 
-    (0 <= idx$) && (idx$ < (R[iir#c] + C[iir#c])) ==> (M[iir#c][idx$ - 0] == (M[iir#b][idx$ - 0] + M[iir#f][idx$ - 0]))
-  );
+  assume 0 <= R[iir#a];
+  assume 0 <= C[iir#a];
+  assume (R[iir#a] + C[iir#a]) == C#init[iir#a];
+  assume 0 <= R[iir#b];
+  assume 0 <= C[iir#b];
+  assume 0 <= R[iir#c];
+  assume 0 <= C[iir#c];
+  assume 0 <= R[iir#d];
+  assume 0 <= C[iir#d];
+  assume 0 <= R[iir#e];
+  assume 0 <= C[iir#e];
+  assume 0 <= R[iir#f];
+  assume 0 <= C[iir#f];
+  assume 0 <= R[iir#g];
+  assume 0 <= C[iir#g];
+  assume R[iir#g] == 0;
+  assume R[iir#e] == ((R[iir#f] + C[iir#f]) - 1);
+  assume R[iir#a] == (R[iir#b] + C[iir#b]);
+  assume R[iir#d] == (R[iir#e] + C[iir#e]);
+  assume R[iir#c] == (R[iir#d] + C[iir#d]);
+  assume R[iir#c] == (R[iir#g] + C[iir#g]);
+  assume R[iir#b] == (R[iir#c] + C[iir#c]);
   assume R[iir#f] == (R[iir#c] + C[iir#c]);
   assume (forall idx$: int :: 
-    (0 <= idx$) && (idx$ < (R[iir#c] + C[iir#c])) ==> (M[iir#c][idx$ - 0] == (M[iir#b][idx$ - 0] + M[iir#f][idx$ - 0]))
+    (1 <= idx$) && (idx$ < (R[iir#f] + C[iir#f])) ==> (M[iir#f][idx$] == M[iir#e][idx$ - 1])
   );
-  assume R[iir#b] == (R[iir#c] + C[iir#c]);
   assume (forall idx$: int :: 
-    (0 <= idx$) && (idx$ < (R[iir#g] + C[iir#g])) ==> (M[iir#g][idx$ - 0] == AT#RShift(M[iir#c][idx$ - 0], 8))
+    (0 <= idx$) && (idx$ < (R[iir#b] + C[iir#b])) ==> (M[iir#b][idx$] == (85 * M[iir#a][idx$]))
   );
-  assume R[iir#c] == (R[iir#g] + C[iir#g]);
   assume (forall idx$: int :: 
-    (0 <= idx$) && (idx$ < (R[iir#d] + C[iir#d])) ==> (M[iir#d][idx$ - 0] == AT#RShift(M[iir#c][idx$ - 0], 8))
+    (0 <= idx$) && (idx$ < (R[iir#e] + C[iir#e])) ==> (M[iir#e][idx$] == (171 * M[iir#d][idx$]))
   );
-  assume R[iir#c] == (R[iir#d] + C[iir#d]);
   assume (forall idx$: int :: 
-    (0 <= idx$) && (idx$ < (R[iir#e] + C[iir#e])) ==> (M[iir#e][idx$ - 0] == (171 * M[iir#d][idx$ - 0]))
+    (0 <= idx$) && (idx$ < (R[iir#d] + C[iir#d])) ==> (M[iir#d][idx$] == AT#RShift(M[iir#c][idx$], 8))
   );
-  assume R[iir#d] == (R[iir#e] + C[iir#e]);
   assume (forall idx$: int :: 
-    (0 <= idx$) && (idx$ < (R[iir#b] + C[iir#b])) ==> (M[iir#b][idx$ - 0] == (85 * M[iir#a][idx$ - 0]))
+    (0 <= idx$) && (idx$ < (R[iir#g] + C[iir#g])) ==> (M[iir#g][idx$] == AT#RShift(M[iir#c][idx$], 8))
   );
-  assume R[iir#a] == (R[iir#b] + C[iir#b]);
   assume (forall idx$: int :: 
-    (0 <= idx$) && (idx$ < ((R[iir#f] + C[iir#f]) - 1)) ==> (M[iir#f][(idx$ + 1) - 0] == M[iir#e][idx$ - 0])
+    (0 <= idx$) && (idx$ < (R[iir#c] + C[iir#c])) ==> (M[iir#c][idx$] == (M[iir#b][idx$] + M[iir#f][idx$]))
   );
-  assume R[iir#e] == ((R[iir#f] + C[iir#f]) - 1);
-  assume R[iir#g] == 0;
-  assume 0 <= C[iir#g];
-  assume 0 <= R[iir#g];
-  assume 0 <= C[iir#f];
-  assume 0 <= R[iir#f];
-  assume 0 <= C[iir#e];
-  assume 0 <= R[iir#e];
-  assume 0 <= C[iir#d];
-  assume 0 <= R[iir#d];
-  assume 0 <= C[iir#c];
-  assume 0 <= R[iir#c];
-  assume 0 <= C[iir#b];
-  assume 0 <= R[iir#b];
-  assume (R[iir#a] + C[iir#a]) == C#init[iir#a];
-  assume 0 <= C[iir#a];
-  assume 0 <= R[iir#a];
   assume (171 * M[iir#g][-1]) == M[iir#f][0];
   assume !(((((1 <= C[iir#e]) || (1 <= C[iir#a])) || (1 <= C[iir#d])) || (1 <= C[iir#c])) || ((1 <= C[iir#b]) && (1 <= C[iir#f])));
   assert {:msg "  23.3: The network might leave unread tokens on channel a"} C[iir#a] == 0;
