tests/Nested.bpl
@@ -1,85 +1,92 @@
-
 // ---------------------------------------------------------------
 // -- Types and global variables ---------------------------------
 // ---------------------------------------------------------------
 type Chan a;
+type Actor;
 type CType = <a>[Chan a]int;
 type MType = <a>[Chan a][int]a;
 type State;
+
 var M: MType;
 var C: CType;
 var R: CType; 
 var C#init: CType;
+var St: [Actor]State;
+
+const unique this#: Actor;
 
 // ---------------------------------------------------------------
 // -- End of prelude ---------------------------------------------
 // ---------------------------------------------------------------
 
+const unique Top#n: Actor;
 const unique Top#x: Chan (int);
 const unique Top#y: Chan (int);
-procedure Top#anon$0#entry()
-  modifies C, R, M;
+procedure Top#anon$0#entry#0()
+  modifies C, R, M, St;
 {
   assume C#init[Top#x] == 1;
   assume C#init[Top#y] == 0;
   assume R[Top#x] == 0;
   assume R[Top#y] == 0;
   assume C#init == C;
-  assert {:msg "  Channel invariant might not hold on action entry"} R[Top#y] == 0;
-  assert {:msg "  Channel invariant might not hold on action entry"} 0 <= C[Top#y];
-  assert {:msg "  Channel invariant might not hold on action entry"} 0 <= R[Top#y];
-  assert {:msg "  Channel invariant might not hold on action entry"} (R[Top#x] + C[Top#x]) == C#init[Top#x];
-  assert {:msg "  Channel invariant might not hold on action entry"} 0 <= C[Top#x];
-  assert {:msg "  Channel invariant might not hold on action entry"} 0 <= R[Top#x];
-  assert {:msg "  4.15: Channel invariant might not hold on action entry"} (R[Top#y] + C[Top#y]) == R[Top#x];
-  assert {:msg "  5.16: Channel invariant might not hold on action entry"} (forall i: int :: 
+  assert {:msg "  Channel invariant might not hold on action entry (generated #0 )"} 0 <= R[Top#x];
+  assert {:msg "  Channel invariant might not hold on action entry (generated #1 )"} 0 <= C[Top#x];
+  assert {:msg "  Channel invariant might not hold on action entry (generated #2 )"} (R[Top#x] + C[Top#x]) == C#init[Top#x];
+  assert {:msg "  Channel invariant might not hold on action entry (generated #3 )"} 0 <= R[Top#y];
+  assert {:msg "  Channel invariant might not hold on action entry (generated #4 )"} 0 <= C[Top#y];
+  assert {:msg "  Channel invariant might not hold on action entry (generated #5 )"} R[Top#y] == 0;
+  assert {:msg "  4.3: Channel invariant might not hold on action entry"} (R[Top#y] + C[Top#y]) == R[Top#x];
+  assert {:msg "  5.3: Channel invariant might not hold on action entry"} (forall i: int :: 
     (0 <= i) && (i < (R[Top#y] + C[Top#y])) ==> (M[Top#x][i] == M[Top#y][i])
   );
 }
-procedure Top#anon$0#Nested#anon$1()
-  modifies C, R, M;
+procedure Top#anon$0#Nested#anon$1#1()
+  modifies C, R, M, St;
 {
+  var St#next: State;
   var x#i: int;
   assume C#init[Top#x] == 1;
   assume C#init[Top#y] == 0;
-  assume R[Top#y] == 0;
-  assume 0 <= C[Top#y];
-  assume 0 <= R[Top#y];
-  assume (R[Top#x] + C[Top#x]) == C#init[Top#x];
-  assume 0 <= C[Top#x];
   assume 0 <= R[Top#x];
+  assume 0 <= C[Top#x];
+  assume (R[Top#x] + C[Top#x]) == C#init[Top#x];
+  assume 0 <= R[Top#y];
+  assume 0 <= C[Top#y];
+  assume R[Top#y] == 0;
   assume (R[Top#y] + C[Top#y]) == R[Top#x];
   assume (forall i: int :: 
     (0 <= i) && (i < (R[Top#y] + C[Top#y])) ==> (M[Top#x][i] == M[Top#y][i])
   );
+  assume true;
   assume 1 <= C[Top#x];
   x#i := M[Top#x][R[Top#x]];
   R[Top#x] := R[Top#x] + 1;
   C[Top#x] := C[Top#x] - 1;
   M[Top#y][R[Top#y] + C[Top#y]] := x#i;
   C[Top#y] := C[Top#y] + 1;
-  assert {:msg "  Sub-actor action at 17.3 might not preserve the channel invariant"} R[Top#y] == 0;
-  assert {:msg "  Sub-actor action at 17.3 might not preserve the channel invariant"} 0 <= C[Top#y];
-  assert {:msg "  Sub-actor action at 17.3 might not preserve the channel invariant"} 0 <= R[Top#y];
-  assert {:msg "  Sub-actor action at 17.3 might not preserve the channel invariant"} (R[Top#x] + C[Top#x]) == C#init[Top#x];
-  assert {:msg "  Sub-actor action at 17.3 might not preserve the channel invariant"} 0 <= C[Top#x];
-  assert {:msg "  Sub-actor action at 17.3 might not preserve the channel invariant"} 0 <= R[Top#x];
-  assert {:msg "  4.15: Sub-actor action at 17.3 might not preserve the channel invariant"} (R[Top#y] + C[Top#y]) == R[Top#x];
-  assert {:msg "  5.16: Sub-actor action at 17.3 might not preserve the channel invariant"} (forall i: int :: 
+  assert {:msg "  Sub-actor action at 17.3 might not preserve the channel invariant (generated #6)"} 0 <= R[Top#x];
+  assert {:msg "  Sub-actor action at 17.3 might not preserve the channel invariant (generated #7)"} 0 <= C[Top#x];
+  assert {:msg "  Sub-actor action at 17.3 might not preserve the channel invariant (generated #8)"} (R[Top#x] + C[Top#x]) == C#init[Top#x];
+  assert {:msg "  Sub-actor action at 17.3 might not preserve the channel invariant (generated #9)"} 0 <= R[Top#y];
+  assert {:msg "  Sub-actor action at 17.3 might not preserve the channel invariant (generated #10)"} 0 <= C[Top#y];
+  assert {:msg "  Sub-actor action at 17.3 might not preserve the channel invariant (generated #11)"} R[Top#y] == 0;
+  assert {:msg "  4.3: Sub-actor action at 17.3 might not preserve the channel invariant"} (R[Top#y] + C[Top#y]) == R[Top#x];
+  assert {:msg "  5.3: Sub-actor action at 17.3 might not preserve the channel invariant"} (forall i: int :: 
     (0 <= i) && (i < (R[Top#y] + C[Top#y])) ==> (M[Top#x][i] == M[Top#y][i])
   );
 }
-procedure Top#anon$0#exit()
-  modifies C, R, M;
+procedure Top#anon$0#exit#2()
+  modifies C, R, M, St;
 {
   assume C#init[Top#x] == 1;
   assume C#init[Top#y] == 0;
-  assume R[Top#y] == 0;
-  assume 0 <= C[Top#y];
-  assume 0 <= R[Top#y];
-  assume (R[Top#x] + C[Top#x]) == C#init[Top#x];
-  assume 0 <= C[Top#x];
   assume 0 <= R[Top#x];
+  assume 0 <= C[Top#x];
+  assume (R[Top#x] + C[Top#x]) == C#init[Top#x];
+  assume 0 <= R[Top#y];
+  assume 0 <= C[Top#y];
+  assume R[Top#y] == 0;
   assume (R[Top#y] + C[Top#y]) == R[Top#x];
   assume (forall i: int :: 
     (0 <= i) && (i < (R[Top#y] + C[Top#y])) ==> (M[Top#x][i] == M[Top#y][i])
@@ -91,71 +98,74 @@ procedure Top#anon$0#exit()
   R[Top#y] := R[Top#y] + C[Top#y];
   C[Top#y] := 0;
 }
+const unique Nested#a: Actor;
 const unique Nested#x: Chan (int);
 const unique Nested#y: Chan (int);
-procedure Nested#anon$1#entry()
-  modifies C, R, M;
+procedure Nested#anon$1#entry#3()
+  modifies C, R, M, St;
 {
   assume C#init[Nested#x] == 1;
   assume C#init[Nested#y] == 0;
   assume R[Nested#x] == 0;
   assume R[Nested#y] == 0;
   assume C#init == C;
-  assert {:msg "  Channel invariant might not hold on action entry"} R[Nested#y] == 0;
-  assert {:msg "  Channel invariant might not hold on action entry"} 0 <= C[Nested#y];
-  assert {:msg "  Channel invariant might not hold on action entry"} 0 <= R[Nested#y];
-  assert {:msg "  Channel invariant might not hold on action entry"} (R[Nested#x] + C[Nested#x]) == C#init[Nested#x];
-  assert {:msg "  Channel invariant might not hold on action entry"} 0 <= C[Nested#x];
-  assert {:msg "  Channel invariant might not hold on action entry"} 0 <= R[Nested#x];
-  assert {:msg "  19.15: Channel invariant might not hold on action entry"} (R[Nested#y] + C[Nested#y]) == R[Nested#x];
-  assert {:msg "  20.16: Channel invariant might not hold on action entry"} (forall i: int :: 
+  assert {:msg "  Channel invariant might not hold on action entry (generated #12 )"} 0 <= R[Nested#x];
+  assert {:msg "  Channel invariant might not hold on action entry (generated #13 )"} 0 <= C[Nested#x];
+  assert {:msg "  Channel invariant might not hold on action entry (generated #14 )"} (R[Nested#x] + C[Nested#x]) == C#init[Nested#x];
+  assert {:msg "  Channel invariant might not hold on action entry (generated #15 )"} 0 <= R[Nested#y];
+  assert {:msg "  Channel invariant might not hold on action entry (generated #16 )"} 0 <= C[Nested#y];
+  assert {:msg "  Channel invariant might not hold on action entry (generated #17 )"} R[Nested#y] == 0;
+  assert {:msg "  19.3: Channel invariant might not hold on action entry"} (R[Nested#y] + C[Nested#y]) == R[Nested#x];
+  assert {:msg "  20.3: Channel invariant might not hold on action entry"} (forall i: int :: 
     (0 <= i) && (i < (R[Nested#y] + C[Nested#y])) ==> (M[Nested#x][i] == M[Nested#y][i])
   );
 }
-procedure Nested#anon$1#Repeater#anon$2()
-  modifies C, R, M;
+procedure Nested#anon$1#Repeater#anon$2#4()
+  modifies C, R, M, St;
 {
+  var St#next: State;
   var in#i: int;
   assume C#init[Nested#x] == 1;
   assume C#init[Nested#y] == 0;
-  assume R[Nested#y] == 0;
-  assume 0 <= C[Nested#y];
-  assume 0 <= R[Nested#y];
-  assume (R[Nested#x] + C[Nested#x]) == C#init[Nested#x];
-  assume 0 <= C[Nested#x];
   assume 0 <= R[Nested#x];
+  assume 0 <= C[Nested#x];
+  assume (R[Nested#x] + C[Nested#x]) == C#init[Nested#x];
+  assume 0 <= R[Nested#y];
+  assume 0 <= C[Nested#y];
+  assume R[Nested#y] == 0;
   assume (R[Nested#y] + C[Nested#y]) == R[Nested#x];
   assume (forall i: int :: 
     (0 <= i) && (i < (R[Nested#y] + C[Nested#y])) ==> (M[Nested#x][i] == M[Nested#y][i])
   );
+  assume true;
   assume 1 <= C[Nested#x];
   in#i := M[Nested#x][R[Nested#x]];
   R[Nested#x] := R[Nested#x] + 1;
   C[Nested#x] := C[Nested#x] - 1;
   M[Nested#y][R[Nested#y] + C[Nested#y]] := in#i;
   C[Nested#y] := C[Nested#y] + 1;
-  assert {:msg "  Sub-actor action at 33.3 might not preserve the channel invariant"} R[Nested#y] == 0;
-  assert {:msg "  Sub-actor action at 33.3 might not preserve the channel invariant"} 0 <= C[Nested#y];
-  assert {:msg "  Sub-actor action at 33.3 might not preserve the channel invariant"} 0 <= R[Nested#y];
-  assert {:msg "  Sub-actor action at 33.3 might not preserve the channel invariant"} (R[Nested#x] + C[Nested#x]) == C#init[Nested#x];
-  assert {:msg "  Sub-actor action at 33.3 might not preserve the channel invariant"} 0 <= C[Nested#x];
-  assert {:msg "  Sub-actor action at 33.3 might not preserve the channel invariant"} 0 <= R[Nested#x];
-  assert {:msg "  19.15: Sub-actor action at 33.3 might not preserve the channel invariant"} (R[Nested#y] + C[Nested#y]) == R[Nested#x];
-  assert {:msg "  20.16: Sub-actor action at 33.3 might not preserve the channel invariant"} (forall i: int :: 
+  assert {:msg "  Sub-actor action at 33.3 might not preserve the channel invariant (generated #18)"} 0 <= R[Nested#x];
+  assert {:msg "  Sub-actor action at 33.3 might not preserve the channel invariant (generated #19)"} 0 <= C[Nested#x];
+  assert {:msg "  Sub-actor action at 33.3 might not preserve the channel invariant (generated #20)"} (R[Nested#x] + C[Nested#x]) == C#init[Nested#x];
+  assert {:msg "  Sub-actor action at 33.3 might not preserve the channel invariant (generated #21)"} 0 <= R[Nested#y];
+  assert {:msg "  Sub-actor action at 33.3 might not preserve the channel invariant (generated #22)"} 0 <= C[Nested#y];
+  assert {:msg "  Sub-actor action at 33.3 might not preserve the channel invariant (generated #23)"} R[Nested#y] == 0;
+  assert {:msg "  19.3: Sub-actor action at 33.3 might not preserve the channel invariant"} (R[Nested#y] + C[Nested#y]) == R[Nested#x];
+  assert {:msg "  20.3: Sub-actor action at 33.3 might not preserve the channel invariant"} (forall i: int :: 
     (0 <= i) && (i < (R[Nested#y] + C[Nested#y])) ==> (M[Nested#x][i] == M[Nested#y][i])
   );
 }
-procedure Nested#anon$1#exit()
-  modifies C, R, M;
+procedure Nested#anon$1#exit#5()
+  modifies C, R, M, St;
 {
   assume C#init[Nested#x] == 1;
   assume C#init[Nested#y] == 0;
-  assume R[Nested#y] == 0;
-  assume 0 <= C[Nested#y];
-  assume 0 <= R[Nested#y];
-  assume (R[Nested#x] + C[Nested#x]) == C#init[Nested#x];
-  assume 0 <= C[Nested#x];
   assume 0 <= R[Nested#x];
+  assume 0 <= C[Nested#x];
+  assume (R[Nested#x] + C[Nested#x]) == C#init[Nested#x];
+  assume 0 <= R[Nested#y];
+  assume 0 <= C[Nested#y];
+  assume R[Nested#y] == 0;
   assume (R[Nested#y] + C[Nested#y]) == R[Nested#x];
   assume (forall i: int :: 
     (0 <= i) && (i < (R[Nested#y] + C[Nested#y])) ==> (M[Nested#x][i] == M[Nested#y][i])
@@ -167,7 +177,8 @@ procedure Nested#anon$1#exit()
   R[Nested#y] := R[Nested#y] + C[Nested#y];
   C[Nested#y] := 0;
 }
-procedure Repeater#anon$2()
+procedure Repeater#anon$2#6()
+  modifies C, R, M, St;
 {
   var i: int;
   assume true;
