tests/Schedule.bpl
@@ -21,7 +21,7 @@ const unique this#: Actor;
 
 const unique FairMerge#s1: State;
 const unique FairMerge#s2: State;
-procedure FairMerge#a1()
+procedure FairMerge#a1#0()
   modifies C, R, M, St;
 {
   var this#: Actor;
@@ -32,7 +32,7 @@ procedure FairMerge#a1()
   St[this#] := FairMerge#s2;
   assert {:msg "  1.1: Action might not preserve invariant"} (St[this#] == FairMerge#s1) || (St[this#] == FairMerge#s2);
 }
-procedure FairMerge#a2()
+procedure FairMerge#a2#1()
   modifies C, R, M, St;
 {
   var this#: Actor;
@@ -47,7 +47,7 @@ const unique Top#fm: Actor;
 const unique Top#a: Chan (int);
 const unique Top#b: Chan (int);
 const unique Top#c: Chan (int);
-procedure Top#anon$0#entry()
+procedure Top#anon$0#entry#2()
   modifies C, R, M, St;
 {
   assume C#init[Top#a] == 1;
@@ -58,25 +58,25 @@ procedure Top#anon$0#entry()
   assume R[Top#c] == 0;
   assume C#init == C;
   assume St[Top#fm] == FairMerge#s1;
-  assert {:msg "  Channel invariant might not hold on action entry"} R[Top#c] == 0;
-  assert {:msg "  Channel invariant might not hold on action entry"} 0 <= C[Top#c];
-  assert {:msg "  Channel invariant might not hold on action entry"} 0 <= R[Top#c];
-  assert {:msg "  Channel invariant might not hold on action entry"} (R[Top#b] + C[Top#b]) == C#init[Top#b];
-  assert {:msg "  Channel invariant might not hold on action entry"} 0 <= C[Top#b];
-  assert {:msg "  Channel invariant might not hold on action entry"} 0 <= R[Top#b];
-  assert {:msg "  Channel invariant might not hold on action entry"} (R[Top#a] + C[Top#a]) == C#init[Top#a];
-  assert {:msg "  Channel invariant might not hold on action entry"} 0 <= C[Top#a];
-  assert {:msg "  Channel invariant might not hold on action entry"} 0 <= R[Top#a];
-  assert {:msg "  16.15: Channel invariant might not hold on action entry"} (R[Top#c] + C[Top#c]) == (R[Top#a] + R[Top#b]);
-  assert {:msg "  17.15: Channel invariant might not hold on action entry"} ((R[Top#c] + C[Top#c]) >= 1) ==> (C[Top#a] == 0);
-  assert {:msg "  18.15: Channel invariant might not hold on action entry"} ((R[Top#c] + C[Top#c]) >= 2) ==> (C[Top#b] == 0);
-  assert {:msg "  19.15: Channel invariant might not hold on action entry"} (R[Top#a] == 0) && (R[Top#b] == 0) ==> (St[Top#fm] == FairMerge#s1);
-  assert {:msg "  20.15: Channel invariant might not hold on action entry"} (R[Top#a] == 1) && (R[Top#b] == 0) ==> (St[Top#fm] == FairMerge#s2);
-  assert {:msg "  21.15: Channel invariant might not hold on action entry"} (R[Top#a] == 1) && (R[Top#b] == 1) ==> (St[Top#fm] == FairMerge#s1);
-  assert {:msg "  23.15: Channel invariant might not hold on action entry"} ((R[Top#c] + C[Top#c]) >= 1) ==> (M[Top#c][0] == M[Top#a][0]);
-  assert {:msg "  24.15: Channel invariant might not hold on action entry"} ((R[Top#c] + C[Top#c]) >= 2) ==> (M[Top#c][1] == M[Top#b][0]);
+  assert {:msg "  Channel invariant might not hold on action entry (generated #0 )"} 0 <= R[Top#a];
+  assert {:msg "  Channel invariant might not hold on action entry (generated #1 )"} 0 <= C[Top#a];
+  assert {:msg "  Channel invariant might not hold on action entry (generated #2 )"} (R[Top#a] + C[Top#a]) == C#init[Top#a];
+  assert {:msg "  Channel invariant might not hold on action entry (generated #3 )"} 0 <= R[Top#b];
+  assert {:msg "  Channel invariant might not hold on action entry (generated #4 )"} 0 <= C[Top#b];
+  assert {:msg "  Channel invariant might not hold on action entry (generated #5 )"} (R[Top#b] + C[Top#b]) == C#init[Top#b];
+  assert {:msg "  Channel invariant might not hold on action entry (generated #6 )"} 0 <= R[Top#c];
+  assert {:msg "  Channel invariant might not hold on action entry (generated #7 )"} 0 <= C[Top#c];
+  assert {:msg "  Channel invariant might not hold on action entry (generated #8 )"} R[Top#c] == 0;
+  assert {:msg "  16.3: Channel invariant might not hold on action entry"} (R[Top#c] + C[Top#c]) == (R[Top#a] + R[Top#b]);
+  assert {:msg "  17.3: Channel invariant might not hold on action entry"} ((R[Top#c] + C[Top#c]) >= 1) ==> (C[Top#a] == 0);
+  assert {:msg "  18.3: Channel invariant might not hold on action entry"} ((R[Top#c] + C[Top#c]) >= 2) ==> (C[Top#b] == 0);
+  assert {:msg "  19.3: Channel invariant might not hold on action entry"} (R[Top#a] == 0) && (R[Top#b] == 0) ==> (St[Top#fm] == FairMerge#s1);
+  assert {:msg "  20.3: Channel invariant might not hold on action entry"} (R[Top#a] == 1) && (R[Top#b] == 0) ==> (St[Top#fm] == FairMerge#s2);
+  assert {:msg "  21.3: Channel invariant might not hold on action entry"} (R[Top#a] == 1) && (R[Top#b] == 1) ==> (St[Top#fm] == FairMerge#s1);
+  assert {:msg "  23.3: Channel invariant might not hold on action entry"} ((R[Top#c] + C[Top#c]) >= 1) ==> (M[Top#c][0] == M[Top#a][0]);
+  assert {:msg "  24.3: Channel invariant might not hold on action entry"} ((R[Top#c] + C[Top#c]) >= 2) ==> (M[Top#c][1] == M[Top#b][0]);
 }
-procedure Top#anon$0#FairMerge#a1()
+procedure Top#anon$0#FairMerge#a1#3()
   modifies C, R, M, St;
 {
   var St#next: State;
@@ -84,15 +84,15 @@ procedure Top#anon$0#FairMerge#a1()
   assume C#init[Top#a] == 1;
   assume C#init[Top#b] == 1;
   assume C#init[Top#c] == 0;
-  assume R[Top#c] == 0;
-  assume 0 <= C[Top#c];
-  assume 0 <= R[Top#c];
-  assume (R[Top#b] + C[Top#b]) == C#init[Top#b];
-  assume 0 <= C[Top#b];
-  assume 0 <= R[Top#b];
-  assume (R[Top#a] + C[Top#a]) == C#init[Top#a];
-  assume 0 <= C[Top#a];
   assume 0 <= R[Top#a];
+  assume 0 <= C[Top#a];
+  assume (R[Top#a] + C[Top#a]) == C#init[Top#a];
+  assume 0 <= R[Top#b];
+  assume 0 <= C[Top#b];
+  assume (R[Top#b] + C[Top#b]) == C#init[Top#b];
+  assume 0 <= R[Top#c];
+  assume 0 <= C[Top#c];
+  assume R[Top#c] == 0;
   assume (R[Top#c] + C[Top#c]) == (R[Top#a] + R[Top#b]);
   assume ((R[Top#c] + C[Top#c]) >= 1) ==> (C[Top#a] == 0);
   assume ((R[Top#c] + C[Top#c]) >= 2) ==> (C[Top#b] == 0);
@@ -110,25 +110,25 @@ procedure Top#anon$0#FairMerge#a1()
   C[Top#c] := C[Top#c] + 1;
   assume St#next == FairMerge#s2;
   St[Top#fm] := St#next;
-  assert {:msg "  Sub-actor action at 2.3 might not preserve the channel invariant"} R[Top#c] == 0;
-  assert {:msg "  Sub-actor action at 2.3 might not preserve the channel invariant"} 0 <= C[Top#c];
-  assert {:msg "  Sub-actor action at 2.3 might not preserve the channel invariant"} 0 <= R[Top#c];
-  assert {:msg "  Sub-actor action at 2.3 might not preserve the channel invariant"} (R[Top#b] + C[Top#b]) == C#init[Top#b];
-  assert {:msg "  Sub-actor action at 2.3 might not preserve the channel invariant"} 0 <= C[Top#b];
-  assert {:msg "  Sub-actor action at 2.3 might not preserve the channel invariant"} 0 <= R[Top#b];
-  assert {:msg "  Sub-actor action at 2.3 might not preserve the channel invariant"} (R[Top#a] + C[Top#a]) == C#init[Top#a];
-  assert {:msg "  Sub-actor action at 2.3 might not preserve the channel invariant"} 0 <= C[Top#a];
-  assert {:msg "  Sub-actor action at 2.3 might not preserve the channel invariant"} 0 <= R[Top#a];
-  assert {:msg "  16.15: Sub-actor action at 2.3 might not preserve the channel invariant"} (R[Top#c] + C[Top#c]) == (R[Top#a] + R[Top#b]);
-  assert {:msg "  17.15: Sub-actor action at 2.3 might not preserve the channel invariant"} ((R[Top#c] + C[Top#c]) >= 1) ==> (C[Top#a] == 0);
-  assert {:msg "  18.15: Sub-actor action at 2.3 might not preserve the channel invariant"} ((R[Top#c] + C[Top#c]) >= 2) ==> (C[Top#b] == 0);
-  assert {:msg "  19.15: Sub-actor action at 2.3 might not preserve the channel invariant"} (R[Top#a] == 0) && (R[Top#b] == 0) ==> (St[Top#fm] == FairMerge#s1);
-  assert {:msg "  20.15: Sub-actor action at 2.3 might not preserve the channel invariant"} (R[Top#a] == 1) && (R[Top#b] == 0) ==> (St[Top#fm] == FairMerge#s2);
-  assert {:msg "  21.15: Sub-actor action at 2.3 might not preserve the channel invariant"} (R[Top#a] == 1) && (R[Top#b] == 1) ==> (St[Top#fm] == FairMerge#s1);
-  assert {:msg "  23.15: Sub-actor action at 2.3 might not preserve the channel invariant"} ((R[Top#c] + C[Top#c]) >= 1) ==> (M[Top#c][0] == M[Top#a][0]);
-  assert {:msg "  24.15: Sub-actor action at 2.3 might not preserve the channel invariant"} ((R[Top#c] + C[Top#c]) >= 2) ==> (M[Top#c][1] == M[Top#b][0]);
+  assert {:msg "  Sub-actor action at 2.3 might not preserve the channel invariant (generated #9)"} 0 <= R[Top#a];
+  assert {:msg "  Sub-actor action at 2.3 might not preserve the channel invariant (generated #10)"} 0 <= C[Top#a];
+  assert {:msg "  Sub-actor action at 2.3 might not preserve the channel invariant (generated #11)"} (R[Top#a] + C[Top#a]) == C#init[Top#a];
+  assert {:msg "  Sub-actor action at 2.3 might not preserve the channel invariant (generated #12)"} 0 <= R[Top#b];
+  assert {:msg "  Sub-actor action at 2.3 might not preserve the channel invariant (generated #13)"} 0 <= C[Top#b];
+  assert {:msg "  Sub-actor action at 2.3 might not preserve the channel invariant (generated #14)"} (R[Top#b] + C[Top#b]) == C#init[Top#b];
+  assert {:msg "  Sub-actor action at 2.3 might not preserve the channel invariant (generated #15)"} 0 <= R[Top#c];
+  assert {:msg "  Sub-actor action at 2.3 might not preserve the channel invariant (generated #16)"} 0 <= C[Top#c];
+  assert {:msg "  Sub-actor action at 2.3 might not preserve the channel invariant (generated #17)"} R[Top#c] == 0;
+  assert {:msg "  16.3: Sub-actor action at 2.3 might not preserve the channel invariant"} (R[Top#c] + C[Top#c]) == (R[Top#a] + R[Top#b]);
+  assert {:msg "  17.3: Sub-actor action at 2.3 might not preserve the channel invariant"} ((R[Top#c] + C[Top#c]) >= 1) ==> (C[Top#a] == 0);
+  assert {:msg "  18.3: Sub-actor action at 2.3 might not preserve the channel invariant"} ((R[Top#c] + C[Top#c]) >= 2) ==> (C[Top#b] == 0);
+  assert {:msg "  19.3: Sub-actor action at 2.3 might not preserve the channel invariant"} (R[Top#a] == 0) && (R[Top#b] == 0) ==> (St[Top#fm] == FairMerge#s1);
+  assert {:msg "  20.3: Sub-actor action at 2.3 might not preserve the channel invariant"} (R[Top#a] == 1) && (R[Top#b] == 0) ==> (St[Top#fm] == FairMerge#s2);
+  assert {:msg "  21.3: Sub-actor action at 2.3 might not preserve the channel invariant"} (R[Top#a] == 1) && (R[Top#b] == 1) ==> (St[Top#fm] == FairMerge#s1);
+  assert {:msg "  23.3: Sub-actor action at 2.3 might not preserve the channel invariant"} ((R[Top#c] + C[Top#c]) >= 1) ==> (M[Top#c][0] == M[Top#a][0]);
+  assert {:msg "  24.3: Sub-actor action at 2.3 might not preserve the channel invariant"} ((R[Top#c] + C[Top#c]) >= 2) ==> (M[Top#c][1] == M[Top#b][0]);
 }
-procedure Top#anon$0#FairMerge#a2()
+procedure Top#anon$0#FairMerge#a2#4()
   modifies C, R, M, St;
 {
   var St#next: State;
@@ -136,15 +136,15 @@ procedure Top#anon$0#FairMerge#a2()
   assume C#init[Top#a] == 1;
   assume C#init[Top#b] == 1;
   assume C#init[Top#c] == 0;
-  assume R[Top#c] == 0;
-  assume 0 <= C[Top#c];
-  assume 0 <= R[Top#c];
-  assume (R[Top#b] + C[Top#b]) == C#init[Top#b];
-  assume 0 <= C[Top#b];
-  assume 0 <= R[Top#b];
-  assume (R[Top#a] + C[Top#a]) == C#init[Top#a];
-  assume 0 <= C[Top#a];
   assume 0 <= R[Top#a];
+  assume 0 <= C[Top#a];
+  assume (R[Top#a] + C[Top#a]) == C#init[Top#a];
+  assume 0 <= R[Top#b];
+  assume 0 <= C[Top#b];
+  assume (R[Top#b] + C[Top#b]) == C#init[Top#b];
+  assume 0 <= R[Top#c];
+  assume 0 <= C[Top#c];
+  assume R[Top#c] == 0;
   assume (R[Top#c] + C[Top#c]) == (R[Top#a] + R[Top#b]);
   assume ((R[Top#c] + C[Top#c]) >= 1) ==> (C[Top#a] == 0);
   assume ((R[Top#c] + C[Top#c]) >= 2) ==> (C[Top#b] == 0);
@@ -162,39 +162,39 @@ procedure Top#anon$0#FairMerge#a2()
   C[Top#c] := C[Top#c] + 1;
   assume St#next == FairMerge#s1;
   St[Top#fm] := St#next;
-  assert {:msg "  Sub-actor action at 3.3 might not preserve the channel invariant"} R[Top#c] == 0;
-  assert {:msg "  Sub-actor action at 3.3 might not preserve the channel invariant"} 0 <= C[Top#c];
-  assert {:msg "  Sub-actor action at 3.3 might not preserve the channel invariant"} 0 <= R[Top#c];
-  assert {:msg "  Sub-actor action at 3.3 might not preserve the channel invariant"} (R[Top#b] + C[Top#b]) == C#init[Top#b];
-  assert {:msg "  Sub-actor action at 3.3 might not preserve the channel invariant"} 0 <= C[Top#b];
-  assert {:msg "  Sub-actor action at 3.3 might not preserve the channel invariant"} 0 <= R[Top#b];
-  assert {:msg "  Sub-actor action at 3.3 might not preserve the channel invariant"} (R[Top#a] + C[Top#a]) == C#init[Top#a];
-  assert {:msg "  Sub-actor action at 3.3 might not preserve the channel invariant"} 0 <= C[Top#a];
-  assert {:msg "  Sub-actor action at 3.3 might not preserve the channel invariant"} 0 <= R[Top#a];
-  assert {:msg "  16.15: Sub-actor action at 3.3 might not preserve the channel invariant"} (R[Top#c] + C[Top#c]) == (R[Top#a] + R[Top#b]);
-  assert {:msg "  17.15: Sub-actor action at 3.3 might not preserve the channel invariant"} ((R[Top#c] + C[Top#c]) >= 1) ==> (C[Top#a] == 0);
-  assert {:msg "  18.15: Sub-actor action at 3.3 might not preserve the channel invariant"} ((R[Top#c] + C[Top#c]) >= 2) ==> (C[Top#b] == 0);
-  assert {:msg "  19.15: Sub-actor action at 3.3 might not preserve the channel invariant"} (R[Top#a] == 0) && (R[Top#b] == 0) ==> (St[Top#fm] == FairMerge#s1);
-  assert {:msg "  20.15: Sub-actor action at 3.3 might not preserve the channel invariant"} (R[Top#a] == 1) && (R[Top#b] == 0) ==> (St[Top#fm] == FairMerge#s2);
-  assert {:msg "  21.15: Sub-actor action at 3.3 might not preserve the channel invariant"} (R[Top#a] == 1) && (R[Top#b] == 1) ==> (St[Top#fm] == FairMerge#s1);
-  assert {:msg "  23.15: Sub-actor action at 3.3 might not preserve the channel invariant"} ((R[Top#c] + C[Top#c]) >= 1) ==> (M[Top#c][0] == M[Top#a][0]);
-  assert {:msg "  24.15: Sub-actor action at 3.3 might not preserve the channel invariant"} ((R[Top#c] + C[Top#c]) >= 2) ==> (M[Top#c][1] == M[Top#b][0]);
+  assert {:msg "  Sub-actor action at 3.3 might not preserve the channel invariant (generated #18)"} 0 <= R[Top#a];
+  assert {:msg "  Sub-actor action at 3.3 might not preserve the channel invariant (generated #19)"} 0 <= C[Top#a];
+  assert {:msg "  Sub-actor action at 3.3 might not preserve the channel invariant (generated #20)"} (R[Top#a] + C[Top#a]) == C#init[Top#a];
+  assert {:msg "  Sub-actor action at 3.3 might not preserve the channel invariant (generated #21)"} 0 <= R[Top#b];
+  assert {:msg "  Sub-actor action at 3.3 might not preserve the channel invariant (generated #22)"} 0 <= C[Top#b];
+  assert {:msg "  Sub-actor action at 3.3 might not preserve the channel invariant (generated #23)"} (R[Top#b] + C[Top#b]) == C#init[Top#b];
+  assert {:msg "  Sub-actor action at 3.3 might not preserve the channel invariant (generated #24)"} 0 <= R[Top#c];
+  assert {:msg "  Sub-actor action at 3.3 might not preserve the channel invariant (generated #25)"} 0 <= C[Top#c];
+  assert {:msg "  Sub-actor action at 3.3 might not preserve the channel invariant (generated #26)"} R[Top#c] == 0;
+  assert {:msg "  16.3: Sub-actor action at 3.3 might not preserve the channel invariant"} (R[Top#c] + C[Top#c]) == (R[Top#a] + R[Top#b]);
+  assert {:msg "  17.3: Sub-actor action at 3.3 might not preserve the channel invariant"} ((R[Top#c] + C[Top#c]) >= 1) ==> (C[Top#a] == 0);
+  assert {:msg "  18.3: Sub-actor action at 3.3 might not preserve the channel invariant"} ((R[Top#c] + C[Top#c]) >= 2) ==> (C[Top#b] == 0);
+  assert {:msg "  19.3: Sub-actor action at 3.3 might not preserve the channel invariant"} (R[Top#a] == 0) && (R[Top#b] == 0) ==> (St[Top#fm] == FairMerge#s1);
+  assert {:msg "  20.3: Sub-actor action at 3.3 might not preserve the channel invariant"} (R[Top#a] == 1) && (R[Top#b] == 0) ==> (St[Top#fm] == FairMerge#s2);
+  assert {:msg "  21.3: Sub-actor action at 3.3 might not preserve the channel invariant"} (R[Top#a] == 1) && (R[Top#b] == 1) ==> (St[Top#fm] == FairMerge#s1);
+  assert {:msg "  23.3: Sub-actor action at 3.3 might not preserve the channel invariant"} ((R[Top#c] + C[Top#c]) >= 1) ==> (M[Top#c][0] == M[Top#a][0]);
+  assert {:msg "  24.3: Sub-actor action at 3.3 might not preserve the channel invariant"} ((R[Top#c] + C[Top#c]) >= 2) ==> (M[Top#c][1] == M[Top#b][0]);
 }
-procedure Top#anon$0#exit()
+procedure Top#anon$0#exit#5()
   modifies C, R, M, St;
 {
   assume C#init[Top#a] == 1;
   assume C#init[Top#b] == 1;
   assume C#init[Top#c] == 0;
-  assume R[Top#c] == 0;
-  assume 0 <= C[Top#c];
-  assume 0 <= R[Top#c];
-  assume (R[Top#b] + C[Top#b]) == C#init[Top#b];
-  assume 0 <= C[Top#b];
-  assume 0 <= R[Top#b];
-  assume (R[Top#a] + C[Top#a]) == C#init[Top#a];
-  assume 0 <= C[Top#a];
   assume 0 <= R[Top#a];
+  assume 0 <= C[Top#a];
+  assume (R[Top#a] + C[Top#a]) == C#init[Top#a];
+  assume 0 <= R[Top#b];
+  assume 0 <= C[Top#b];
+  assume (R[Top#b] + C[Top#b]) == C#init[Top#b];
+  assume 0 <= R[Top#c];
+  assume 0 <= C[Top#c];
+  assume R[Top#c] == 0;
   assume (R[Top#c] + C[Top#c]) == (R[Top#a] + R[Top#b]);
   assume ((R[Top#c] + C[Top#c]) >= 1) ==> (C[Top#a] == 0);
   assume ((R[Top#c] + C[Top#c]) >= 2) ==> (C[Top#b] == 0);
@@ -211,5 +211,5 @@ procedure Top#anon$0#exit()
   assert {:msg "  12.38: Network output might not conform to specified action output"} M[Top#c][1] == M[Top#b][0];
   R[Top#c] := R[Top#c] + C[Top#c];
   C[Top#c] := 0;
-  assert {:msg "  14.13: The network might not preserve the network invariant"} St[Top#fm] == FairMerge#s1;
+  assert {:msg "  14.3: The network might not preserve the network invariant"} St[Top#fm] == FairMerge#s1;
 }
