tests/MultiInMultiOut.bpl
@@ -1,0 +1,147 @@
+// ---------------------------------------------------------------
+// -- Types and global variables ---------------------------------
+// ---------------------------------------------------------------
+type Chan a;
+type Actor;
+type CType = <a>[Chan a]int;
+type MType = <a>[Chan a][int]a;
+type State;
+
+var M: MType;
+var C: CType;
+var R: CType; 
+var C#init: CType;
+var St: [Actor]State;
+
+const unique this#: Actor;
+
+function AT#Abs(x: int): int { if 0 <= x then x else -x }
+function AT#Div(int, int): int;
+function AT#Mod(int, int): int;
+axiom (forall a,b: int :: AT#Div(a,b)*b + AT#Mod(a,b) == a);
+axiom (forall a,b: int :: 0 <= AT#Mod(a,b) && AT#Mod(a,b) < AT#Abs(b));
+
+// ---------------------------------------------------------------
+// -- End of prelude ---------------------------------------------
+// ---------------------------------------------------------------
+
+procedure Test#anon$0#0()
+  modifies C, R, M, St;
+{
+  var i: int;
+  var j: int;
+  assume true;
+}
+const unique Net#t: Actor;
+const unique Net#a: Chan (int);
+const unique Net#b: Chan (int);
+procedure Net#anon$1#entry#1()
+  modifies C, R, M, St;
+{
+  assume C#init[Net#a] == 2;
+  assume C#init[Net#b] == 0;
+  assume R[Net#a] == 0;
+  assume R[Net#b] == 0;
+  assume C#init == C;
+  assert {:msg "  Channel invariant might not hold on action entry (generated #0 )"} 0 <= R[Net#a];
+  assert {:msg "  Channel invariant might not hold on action entry (generated #1 )"} 0 <= C[Net#a];
+  assert {:msg "  Channel invariant might not hold on action entry (generated #2 )"} (R[Net#a] + C[Net#a]) == C#init[Net#a];
+  assert {:msg "  Channel invariant might not hold on action entry (generated #3 )"} 0 <= R[Net#b];
+  assert {:msg "  Channel invariant might not hold on action entry (generated #4 )"} 0 <= C[Net#b];
+  assert {:msg "  Channel invariant might not hold on action entry (generated #5 )"} R[Net#b] == 0;
+  assert {:msg "  Channel invariant might not hold on action entry (generated #6 )"} (3 * R[Net#a]) == (2 * (R[Net#b] + C[Net#b]));
+  assert {:msg "  Channel invariant might not hold on action entry (generated #7 )"} (forall idx$: int :: 
+    (0 <= idx$) && (idx$ < (R[Net#b] + C[Net#b])) && (AT#Mod(idx$, 3) == 0) ==> (M[Net#b][idx$] == (M[Net#a][AT#Div(2, 3) * idx$] + M[Net#a][(AT#Div(2, 3) * idx$) + 1]))
+  );
+  assert {:msg "  Channel invariant might not hold on action entry (generated #8 )"} (forall idx$: int :: 
+    (0 <= idx$) && (idx$ < (R[Net#b] + C[Net#b])) && (AT#Mod(idx$, 3) == 1) ==> (M[Net#b][idx$] == (M[Net#a][AT#Div(2, 3) * idx$] - M[Net#a][(AT#Div(2, 3) * idx$) + 1]))
+  );
+  assert {:msg "  Channel invariant might not hold on action entry (generated #9 )"} (forall idx$: int :: 
+    (0 <= idx$) && (idx$ < (R[Net#b] + C[Net#b])) && (AT#Mod(idx$, 3) == 2) ==> (M[Net#b][idx$] == (M[Net#a][AT#Div(2, 3) * idx$] * M[Net#a][(AT#Div(2, 3) * idx$) + 1]))
+  );
+}
+procedure Net#anon$1#Test#anon$0#2()
+  modifies C, R, M, St;
+{
+  var St#next: State;
+  var in#i: int;
+  var in#j: int;
+  assume C#init[Net#a] == 2;
+  assume C#init[Net#b] == 0;
+  assume 0 <= R[Net#a];
+  assume 0 <= C[Net#a];
+  assume (R[Net#a] + C[Net#a]) == C#init[Net#a];
+  assume 0 <= R[Net#b];
+  assume 0 <= C[Net#b];
+  assume R[Net#b] == 0;
+  assume (3 * R[Net#a]) == (2 * (R[Net#b] + C[Net#b]));
+  assume (forall idx$: int :: 
+    (0 <= idx$) && (idx$ < (R[Net#b] + C[Net#b])) && (AT#Mod(idx$, 3) == 0) ==> (M[Net#b][idx$] == (M[Net#a][AT#Div(2, 3) * idx$] + M[Net#a][(AT#Div(2, 3) * idx$) + 1]))
+  );
+  assume (forall idx$: int :: 
+    (0 <= idx$) && (idx$ < (R[Net#b] + C[Net#b])) && (AT#Mod(idx$, 3) == 1) ==> (M[Net#b][idx$] == (M[Net#a][AT#Div(2, 3) * idx$] - M[Net#a][(AT#Div(2, 3) * idx$) + 1]))
+  );
+  assume (forall idx$: int :: 
+    (0 <= idx$) && (idx$ < (R[Net#b] + C[Net#b])) && (AT#Mod(idx$, 3) == 2) ==> (M[Net#b][idx$] == (M[Net#a][AT#Div(2, 3) * idx$] * M[Net#a][(AT#Div(2, 3) * idx$) + 1]))
+  );
+  assume true;
+  assume 2 <= C[Net#a];
+  in#i := M[Net#a][R[Net#a]];
+  R[Net#a] := R[Net#a] + 1;
+  C[Net#a] := C[Net#a] - 1;
+  in#j := M[Net#a][R[Net#a]];
+  R[Net#a] := R[Net#a] + 1;
+  C[Net#a] := C[Net#a] - 1;
+  M[Net#b][R[Net#b] + C[Net#b]] := in#i + in#j;
+  C[Net#b] := C[Net#b] + 1;
+  M[Net#b][R[Net#b] + C[Net#b]] := in#i - in#j;
+  C[Net#b] := C[Net#b] + 1;
+  M[Net#b][R[Net#b] + C[Net#b]] := in#i * in#j;
+  C[Net#b] := C[Net#b] + 1;
+  assert {:msg "  Sub-actor action at 3.3 might not preserve the channel invariant (generated #10)"} 0 <= R[Net#a];
+  assert {:msg "  Sub-actor action at 3.3 might not preserve the channel invariant (generated #11)"} 0 <= C[Net#a];
+  assert {:msg "  Sub-actor action at 3.3 might not preserve the channel invariant (generated #12)"} (R[Net#a] + C[Net#a]) == C#init[Net#a];
+  assert {:msg "  Sub-actor action at 3.3 might not preserve the channel invariant (generated #13)"} 0 <= R[Net#b];
+  assert {:msg "  Sub-actor action at 3.3 might not preserve the channel invariant (generated #14)"} 0 <= C[Net#b];
+  assert {:msg "  Sub-actor action at 3.3 might not preserve the channel invariant (generated #15)"} R[Net#b] == 0;
+  assert {:msg "  Sub-actor action at 3.3 might not preserve the channel invariant (generated #16)"} (3 * R[Net#a]) == (2 * (R[Net#b] + C[Net#b]));
+  assert {:msg "  Sub-actor action at 3.3 might not preserve the channel invariant (generated #17)"} (forall idx$: int :: 
+    (0 <= idx$) && (idx$ < (R[Net#b] + C[Net#b])) && (AT#Mod(idx$, 3) == 0) ==> (M[Net#b][idx$] == (M[Net#a][AT#Div(2, 3) * idx$] + M[Net#a][(AT#Div(2, 3) * idx$) + 1]))
+  );
+  assert {:msg "  Sub-actor action at 3.3 might not preserve the channel invariant (generated #18)"} (forall idx$: int :: 
+    (0 <= idx$) && (idx$ < (R[Net#b] + C[Net#b])) && (AT#Mod(idx$, 3) == 1) ==> (M[Net#b][idx$] == (M[Net#a][AT#Div(2, 3) * idx$] - M[Net#a][(AT#Div(2, 3) * idx$) + 1]))
+  );
+  assert {:msg "  Sub-actor action at 3.3 might not preserve the channel invariant (generated #19)"} (forall idx$: int :: 
+    (0 <= idx$) && (idx$ < (R[Net#b] + C[Net#b])) && (AT#Mod(idx$, 3) == 2) ==> (M[Net#b][idx$] == (M[Net#a][AT#Div(2, 3) * idx$] * M[Net#a][(AT#Div(2, 3) * idx$) + 1]))
+  );
+}
+procedure Net#anon$1#exit#3()
+  modifies C, R, M, St;
+{
+  assume C#init[Net#a] == 2;
+  assume C#init[Net#b] == 0;
+  assume 0 <= R[Net#a];
+  assume 0 <= C[Net#a];
+  assume (R[Net#a] + C[Net#a]) == C#init[Net#a];
+  assume 0 <= R[Net#b];
+  assume 0 <= C[Net#b];
+  assume R[Net#b] == 0;
+  assume (3 * R[Net#a]) == (2 * (R[Net#b] + C[Net#b]));
+  assume (forall idx$: int :: 
+    (0 <= idx$) && (idx$ < (R[Net#b] + C[Net#b])) && (AT#Mod(idx$, 3) == 0) ==> (M[Net#b][idx$] == (M[Net#a][AT#Div(2, 3) * idx$] + M[Net#a][(AT#Div(2, 3) * idx$) + 1]))
+  );
+  assume (forall idx$: int :: 
+    (0 <= idx$) && (idx$ < (R[Net#b] + C[Net#b])) && (AT#Mod(idx$, 3) == 1) ==> (M[Net#b][idx$] == (M[Net#a][AT#Div(2, 3) * idx$] - M[Net#a][(AT#Div(2, 3) * idx$) + 1]))
+  );
+  assume (forall idx$: int :: 
+    (0 <= idx$) && (idx$ < (R[Net#b] + C[Net#b])) && (AT#Mod(idx$, 3) == 2) ==> (M[Net#b][idx$] == (M[Net#a][AT#Div(2, 3) * idx$] * M[Net#a][(AT#Div(2, 3) * idx$) + 1]))
+  );
+  assume !(2 <= C[Net#a]);
+  assert {:msg "  7.3: The network might leave unread tokens on channel a"} C[Net#a] == 0;
+  assert {:msg "  7.3: The network might not produce the specified number of tokens on output out"} C[Net#b] == 3;
+  assert {:msg "  7.28: Network output might not conform to specified action output"} M[Net#b][0] == (M[Net#a][0] + M[Net#a][1]);
+  assert {:msg "  7.32: Network output might not conform to specified action output"} M[Net#b][1] == (M[Net#a][0] - M[Net#a][1]);
+  assert {:msg "  7.36: Network output might not conform to specified action output"} M[Net#b][2] == (M[Net#a][0] * M[Net#a][1]);
+  R[Net#b] := R[Net#b] + C[Net#b];
+  C[Net#b] := 0;
+}
